working commit

coq/Scheduler/Contract.v
@@ -34,6 +34,18 @@ Record TFSchedContext := {
   tfs_spec_action_ops : tfs_spec_action -> @tf_ops tfs_spec_states tfs_spec_inputs tfs_spec_outputs
 }.
 
+Inductive _tfs_ops_t {s_t o_t} :=
+  | StOp (s: s_t)
+  | OutOp (o: o_t).
+
+Definition tfs_ops_no_duplicates {s i o} (ops: list (@tf_op s i o)) : Prop :=
+  NoDup (flat_map (fun op => 
+    match op with 
+      | tf_assign dst _ => [StOp dst]  
+      | tf_output dst _ => [OutOp dst]
+      | _ => []
+    end) ops).
+
 Record TFSchedule := {
   tfs_ctx: TFSchedContext;
 
@@ -59,10 +71,128 @@ Record TFSchedule := {
   tfs_map_to: ((ContextEnv (FT:=(tfs_spec_states_fin tfs_ctx))).(env_t) (tf_states_type (tfs_spec_states_size tfs_ctx))) -> ((ContextEnv (FT:=tfs_states_fin)).(env_t) (tf_states_type tfs_states_size));
   tfs_map_from: ((ContextEnv (FT:=tfs_states_fin)).(env_t) (tf_states_type tfs_states_size)) -> ((ContextEnv (FT:=(tfs_spec_states_fin tfs_ctx))).(env_t) (tf_states_type (tfs_spec_states_size tfs_ctx)));
 
-  (* returns the actions that should always run (fst) and the actions that should only run when the done signal is set (snd) *)
+  (* returns the operations that should always run (fst) and the operations that should only run when the done signal is set (snd) *)
   tfs_schedule: tfs_action -> list (@tf_op tfs_states tfs_inputs tfs_outputs) * list (@tf_op tfs_states tfs_inputs tfs_outputs);
   (* after the done signal is set, the next cycle the module is ready for new input & the modules output is valid (if the above schedule is respected) *)
   tfs_done_signal: tfs_states;
-  (* these states have to be reset if the done signal is set *)
+  (* these states have to be reset to Bits.zero if the done signal is set *)
   tfs_reset_states: list tfs_states;
+
+  tfs_schedule_no_duplicates: forall a, tfs_ops_no_duplicates (fst (tfs_schedule a) ++ snd (tfs_schedule a));
 }.
+
+Section SchedulerSpec.
+
+  Context (tf_sched_ctx : TFSchedule).
+
+  Local Notation s_var := (tfs_states tf_sched_ctx).
+  Local Notation i_var := (tfs_inputs tf_sched_ctx).
+  Local Notation o_var := (tfs_outputs tf_sched_ctx).
+  Local Notation s_sz := (tfs_states_size tf_sched_ctx).
+  Local Notation i_sz := (tfs_inputs_size tf_sched_ctx).
+  Local Notation o_sz := (tfs_outputs_size tf_sched_ctx).
+  
+  Local Notation st_env := (ContextEnv.(env_t) (tf_states_type s_sz)).
+  Local Notation out_env := (ContextEnv.(env_t) (tf_outputs_type o_sz)).
+  Local Notation sys_state_t := (st_env * out_env)%type.
+  Local Notation input_t := (forall x : i_var, type_denote (tf_inputs_type i_sz x)).
+
+  Hint Extern 0 (FiniteType s_var) => exact (tfs_states_fin (tf_sched_ctx)) : typeclass_instances.
+  Hint Extern 0 (FiniteType i_var) => exact (tfs_inputs_fin (tf_sched_ctx)) : typeclass_instances.
+  Hint Extern 0 (FiniteType o_var) => exact (tfs_outputs_fin (tf_sched_ctx)) : typeclass_instances.
+
+  Definition tfs_get_updates
+    (ops: list (@tf_op s_var i_var o_var))
+    (sys_state: sys_state_t)
+    (input: input_t) :=
+    List.map (fun op => tf_op_step_updates s_sz i_sz o_sz op sys_state input) ops.
+
+  (* Definition tfs_reset_states_list
+    (states_to_reset: list s_var)
+    (sys_state: sys_state_t)
+    : sys_state_t :=
+    List.fold_left (fun (st : sys_state_t) (v : s_var) =>
+      let st_env' := ContextEnv.(putenv) (fst st) v (tfs_states_init tf_sched_ctx v) in
+      (st_env', snd st)
+    ) states_to_reset sys_state. *)
+
+  Definition tfs_reset_updates
+    (states_to_reset: list s_var)
+    :=
+    List.map (fun v => tf_st_update s_sz o_sz v (tfs_states_init tf_sched_ctx v)) states_to_reset.
+
+  (* Definition tfs_commit_updates
+    updates
+    (sys_state: sys_state_t)
+    : sys_state_t :=
+    List.fold_left (fun (st : sys_state_t) u => tf_op_step_commit s_sz o_sz st u) updates sys_state. *)
+
+  Fixpoint find_st_update (x: s_var) (ups: list (tf_update s_sz o_sz)) : option (bits_t (s_sz x)) :=
+    match ups with
+    | nil => None
+    | u :: rest =>
+        match u with
+        | tf_st_update _ _ var val =>
+            match eq_dec var x with
+            | left eq_proof => 
+                Some (match eq_proof in (_ = y) return bits_t (s_sz y) with
+                      | eq_refl => val
+                      end)
+            | right _ => find_st_update x rest
+            end
+        | _ => find_st_update x rest
+        end
+    end.
+
+  Definition find_st_val (x: s_var) (ups: list (tf_update s_sz o_sz)) (sys_state: sys_state_t) : bits_t (s_sz x) :=
+    match find_st_update x ups with
+    | Some v => v
+    | None => (fst sys_state).[x]
+    end.
+
+  Fixpoint find_out_update (x: o_var) (ups: list (tf_update s_sz o_sz)) : option (bits_t (o_sz x)) :=
+    match ups with
+    | nil => None
+    | u :: rest =>
+        match u with
+        | tf_out_update _ _ var val =>
+            match eq_dec var x with
+            | left eq_proof => 
+                Some (match eq_proof in (_ = y) return bits_t (o_sz y) with
+                      | eq_refl => val
+                      end)
+            | right _ => find_out_update x rest
+            end
+        | _ => find_out_update x rest
+        end
+    end.
+
+  Definition find_out_val (x: o_var) (ups: list (tf_update s_sz o_sz)) (sys_state: sys_state_t) : bits_t (o_sz x) :=
+    match find_out_update x ups with
+    | Some v => v
+    | None => (snd sys_state).[x]
+    end.
+
+  Definition tfs_next_cycle
+    (action: tfs_action tf_sched_ctx)
+    (sys_state: sys_state_t)
+    (input: input_t)
+    : sys_state_t :=
+    let always_ops := fst (tfs_schedule tf_sched_ctx action) in
+    let done_ops := snd (tfs_schedule tf_sched_ctx action) in
+
+    (* Evaluate ALL updates based on the clean initial cycle state *)
+    let always_updates := tfs_get_updates always_ops sys_state input in
+    let done_updates := tfs_get_updates done_ops sys_state input in
+    let reset_updates := tfs_reset_updates (tfs_reset_states tf_sched_ctx) in
+     
+    let done_val := find_st_val (tfs_done_signal tf_sched_ctx) always_updates sys_state in
+
+    let updates := if beq_dec done_val Bits.zero then always_updates else (reset_updates ++ done_updates ++ always_updates) in
+
+    ( 
+      ContextEnv.(create) (fun x => find_st_val x updates sys_state),
+      ContextEnv.(create) (fun x => find_out_val x updates sys_state)
+    ).
+
+End SchedulerSpec.
