coq/Examples/SchedExample.v
@@ -1,0 +1,173 @@
+Require Import Koika.Frontend.
+Require Import Koika.Std.
+Require Koika.KoikaForm.Untyped.UntypedSemantics.
+Require Import Koika.KoikaForm.SimpleVal.
+
+Require Import Trustformer.Syntax.
+Require Import Trustformer.Semantics.
+Require Import Trustformer.TypedSynthesis.
+Require Import Trustformer.Scheduler.Contract.
+Require Import Trustformer.Scheduler.VariableScheduler.
+
+Require Import Coq.Logic.EqdepFacts.
+
+Require Import Hammer.Plugin.Hammer.
+Set Hammer GSMode 63.
+
+(*
+    An example specification and synthesis of a simple lockbox.
+    The hardware module has a single internal state register (32 bits) and supports two actions (set, test).
+    Actions are triggered through a command register, where the first 1 bit indicates if the command is valid,
+    and the remaining bits indicate the action to perform.
+
+ *)
+
+Section FunctionalSpecification.
+
+    Definition sz := 32.
+
+    Inductive fs_action :=
+    | fs_act
+    .
+
+    Definition fs_action_encoding (a: fs_action) : bits_t 16 :=
+    match a with
+    | fs_act => Bits.of_nat 16 10
+    end.
+
+    Lemma fs_action_encoding_inj :
+        forall a1 a2,
+        fs_action_encoding a1 = fs_action_encoding a2 ->
+        a1 = a2.
+    Proof.
+        intros. unfold fs_action_encoding in H.
+        destruct a1; destruct a2; try reflexivity; try discriminate.
+    Qed.
+
+    Inductive fs_states :=
+    | x
+    | y
+    .
+
+    Inductive fs_inputs :=
+    | in_A
+    .
+
+    Inductive fs_outputs :=
+    | out_A
+    .
+
+    Definition fs_states_size (x: fs_states) : nat :=
+    sz.
+
+    Definition fs_inputs_size (x: fs_inputs) : nat := 
+    sz.
+
+    Definition fs_outputs_size (x: fs_outputs) : nat := 
+    sz.
+
+    Definition fs_states_t := tf_states_type fs_states_size. 
+
+    Definition fs_states_init (x: fs_states) : (fs_states_t x) :=
+        match x with
+        | x => Bits.zero
+        | y => Bits.zero
+        end.
+
+    Definition fs_transitions
+        (act: fs_action)
+        :
+        (@tf_ops fs_states fs_inputs fs_outputs)
+        :=
+        match act with
+        | fs_act => 
+            {[
+                let $x := $x * $x;
+                (if $in_A then
+                    let $y := $x * $y;
+                    let $x := $x + #1
+                else
+                    pass
+                );
+                let $out_A := $y 
+            ]}
+        end.
+
+    Definition fs_step := tf_ops_run fs_states_size fs_inputs_size fs_outputs_size.
+    
+    Section Examples.
+        
+
+    End Examples.
+
+End FunctionalSpecification.
+
+
+Section TypedSynthesis.
+
+    Definition tfs_ctx : TFSchedContext := {|
+        tfs_spec_states := fs_states;
+        tfs_spec_states_fin := _;
+        tfs_spec_states_size := fs_states_size;
+        tfs_spec_states_init := fs_states_init;
+
+        tfs_spec_inputs := fs_inputs;
+        tfs_spec_inputs_fin := _;
+        tfs_spec_inputs_size := fs_inputs_size;
+
+        tfs_spec_outputs := fs_outputs;
+        tfs_spec_outputs_fin := _;
+        tfs_spec_outputs_size := fs_outputs_size;
+
+        tfs_spec_action := fs_action;
+        tfs_spec_action_fin := _;
+        tfs_spec_action_ops := fs_transitions
+    |}.
+
+    Definition tf_schedule := tfs_schedule tfs_ctx 5.
+
+    Definition tf_ctx : TFSynthContext := {|
+        tf_sched_ctx := tf_schedule;
+
+        tf_action_encoding := fs_action_encoding;
+        tf_action_encoding_inj := fs_action_encoding_inj;
+    |}.
+
+    Definition R := TypedSynthesis.R tf_ctx.
+
+    Definition r := TypedSynthesis.r tf_ctx.
+
+    Definition Sigma := TypedSynthesis.Sigma tf_ctx.
+
+    Definition system_schedule := TypedSynthesis.system_schedule tf_ctx.
+    
+    Definition ext_fn_specs := TypedSynthesis.ext_fn_specs tf_ctx.
+
+    Instance ext_fn_names : Show _ := TypedSynthesis.ext_fn_names tf_ctx.
+
+    Definition package :=
+      {| ip_koika := {| koika_reg_types := R;
+                        koika_reg_names := TypedSynthesis.reg_names tf_ctx;
+                        koika_reg_init := r;
+                        koika_reg_finite := TypedSynthesis._reg_t_finite tf_ctx;
+                        koika_ext_fn_types := Sigma;
+                        koika_rules := TypedSynthesis.rules tf_ctx;
+                        koika_rule_names := TypedSynthesis.rule_names tf_ctx;
+                        koika_rule_external := (fun _ => false);
+                        koika_scheduler := system_schedule;
+                        koika_module_name := "Example_Sched" |};
+
+      ip_sim := {| sp_ext_fn_specs fn := {| efs_name := show fn; efs_method := false |};
+                  sp_prelude := None |};
+
+      ip_verilog := {| vp_ext_fn_specs := ext_fn_specs |} |}.
+    
+
+End TypedSynthesis.
+
+(* Extraction *)
+
+Definition prog := Interop.Backends.register package.
+Set Extraction Output Directory "build".
+Extraction "Example_Sched.ml" prog.
+
