coq/Properties/Common.v
@@ -13,601 +13,742 @@ Require Import Hammer.Plugin.Hammer.
 Set Hammer GSMode 63.
 
 Section Logs.
-    Context {V: Type}.
+  Context {V: Type}.
 
-    Context {reg_t: Type}.
-    Context {REnv: Env reg_t}.
-    Definition R : reg_t -> Type := fun _ => V.
+  Context {reg_t: Type}.
+  Context {REnv: Env reg_t}.
+  Definition R : reg_t -> Type := fun _ => V.
 
-    Notation Log := (@_ULog V reg_t REnv).
+  Notation Log := (@_ULog V reg_t REnv).
 
-    Lemma log_find_empty {T} idx (f: @LogEntry (R idx) -> option T):
-        log_find (log_empty: Log) idx f = None.
-    Proof.
-        unfold log_find, log_empty; intros; rewrite getenv_create; reflexivity.
-    Qed.
+  Lemma ulog_find_empty {T} idx (f: @LogEntry (R idx) -> option T):
+    log_find (log_empty: Log) idx f = None.
+  Proof.
+    unfold log_find, log_empty; intros; rewrite getenv_create; reflexivity.
+  Qed.
 
-    Lemma log_app_assoc : forall (l1 l2 l3: Log),
-        log_app (log_app l1 l2) l3 = log_app l1 (log_app l2 l3).
-    Proof.
-        unfold log_app, map2; intros.
-        apply create_funext. intros.
-        rewrite !getenv_create.
-        rewrite app_assoc.
-        reflexivity.
-    Qed.
+  Lemma ulog_app_assoc : forall (l1 l2 l3: Log),
+    log_app (log_app l1 l2) l3 = log_app l1 (log_app l2 l3).
+  Proof.
+    unfold log_app, map2; intros.
+    apply create_funext. intros.
+    rewrite !getenv_create.
+    rewrite app_assoc.
+    reflexivity.
+  Qed.
 
-    Lemma log_app_empty_l : forall (l: Log),
-        log_app log_empty l = l.
-    Proof.
-        intros.
-        apply equiv_eq.
-        unfold equiv, log_app, map2, log_empty; intros.
-        rewrite !getenv_create, app_nil_l.
-        reflexivity.
-    Qed.
+  Lemma ulog_app_empty_l : forall (l: Log),
+    log_app log_empty l = l.
+  Proof.
+    intros.
+    apply equiv_eq.
+    unfold equiv, log_app, map2, log_empty; intros.
+    rewrite !getenv_create, app_nil_l.
+    reflexivity.
+  Qed.
 
-    Lemma log_app_empty_r : forall (l: Log),
-        log_app l log_empty = l.
-    Proof.
-        intros.
-        apply equiv_eq.
-        unfold equiv, log_app, map2, log_empty; intros.
-        rewrite !getenv_create, app_nil_r.
-        reflexivity.
-    Qed.
+  Lemma ulog_app_empty_r : forall (l: Log),
+    log_app l log_empty = l.
+  Proof.
+    intros.
+    apply equiv_eq.
+    unfold equiv, log_app, map2, log_empty; intros.
+    rewrite !getenv_create, app_nil_r.
+    reflexivity.
+  Qed.
 
-    Lemma log_existsb_empty:
-        forall p idx,
-        log_existsb (log_empty: Log) idx p = false.
-    Proof.
-        unfold log_existsb, log_empty; intros.
-        rewrite getenv_create.
-        reflexivity.
-    Qed.
+  Lemma ulog_existsb_empty:
+    forall p idx,
+    log_existsb (log_empty: Log) idx p = false.
+  Proof.
+    unfold log_existsb, log_empty; intros.
+    rewrite getenv_create.
+    reflexivity.
+  Qed.
 End Logs.
 
 Section FiniteType.
 
-    Context {T: Type}.
-    Context {fin_t: FiniteType T}.
+  Context {T: Type}.
+  Context {fin_t: FiniteType T}.
 
-    Lemma finite_index_bounded (x: T):
-        (finite_index x < List.length (finite_elements))%nat.
-    Proof.
-        generalize (finite_surjective x). intros H.
-        apply nth_error_Some. (* hammer. *) sfirstorder.
-    Qed.
+  Lemma finite_index_bounded (x: T):
+    (finite_index x < List.length (finite_elements))%nat.
+  Proof.
+    generalize (finite_surjective x). intros H.
+    apply nth_error_Some. (* hammer. *) sfirstorder.
+  Qed.
 
-    Lemma finite_elements_is_finfun_listing:
-        FinFun.Listing finite_elements.
-    Proof.
-        unfold FinFun.Listing.
-        split.
-        - apply finite_nodup.
-        - unfold FinFun.Full.
-          intros x.
-          generalize (finite_surjective x). intros H.
-          apply (nth_error_In finite_elements (finite_index x)). (* hammer. *) sfirstorder.
-    Qed.
+  Lemma finite_elements_is_finfun_listing:
+    FinFun.Listing finite_elements.
+  Proof.
+    unfold FinFun.Listing.
+    split.
+    - apply finite_nodup.
+    - unfold FinFun.Full.
+      intros x.
+      generalize (finite_surjective x). intros H.
+      apply (nth_error_In finite_elements (finite_index x)). (* hammer. *) sfirstorder.
+  Qed.
 
-    Lemma finite_index_finfun_inj: 
-        FinFun.Injective finite_index.
-    Proof.
-        unfold FinFun.Injective. exact finite_index_injective.
-    Qed.
+  Lemma finite_index_finfun_inj: 
+    FinFun.Injective finite_index.
+  Proof.
+    unfold FinFun.Injective. exact finite_index_injective.
+  Qed.
 
-    Lemma finite_index_plus_constant_r_inj:
-        forall c x y,
-        finite_index x + c = finite_index y + c ->
-        x = y.
-    Proof.
-        intros. generalize (finite_index_injective x y). intros.
-        apply Nat.add_cancel_r in H. (* hammer. *) sfirstorder.
-    Qed.
+  Lemma finite_index_plus_constant_r_inj:
+    forall c x y,
+    finite_index x + c = finite_index y + c ->
+    x = y.
+  Proof.
+    intros. generalize (finite_index_injective x y). intros.
+    apply Nat.add_cancel_r in H. (* hammer. *) sfirstorder.
+  Qed.
 
-    Lemma finite_index_plus_constant_l_inj:
-        forall c x y,
-        c + finite_index x = c + finite_index y ->
-        x = y.
-    Proof.
-        intros. generalize (finite_index_injective x y). intros.
-        apply Nat.add_cancel_l in H. (* hammer. *) sfirstorder.
-    Qed.
+  Lemma finite_index_plus_constant_l_inj:
+    forall c x y,
+    c + finite_index x = c + finite_index y ->
+    x = y.
+  Proof.
+    intros. generalize (finite_index_injective x y). intros.
+    apply Nat.add_cancel_l in H. (* hammer. *) sfirstorder.
+  Qed.
 
 End FiniteType.
 
 Section Schedule.
 
-    Context {pos_t rule_name_t: Type}.
-    Context {rule_name_t_eq_dec: EqDec rule_name_t}.
-    Definition sched := @scheduler pos_t rule_name_t.
+  Context {pos_t rule_name_t: Type}.
+  Context {rule_name_t_eq_dec: EqDec rule_name_t}.
+  Definition sched := @scheduler pos_t rule_name_t.
 
-    Fixpoint scheduler_has_rule (scheduler : sched) (r_target : rule_name_t) : Prop :=
-        match scheduler with
-        | Done => False
-        | Cons r s => if eq_dec r r_target then True else scheduler_has_rule s r_target
-        | Try r s1 s2 => if eq_dec r r_target then True else (scheduler_has_rule s1 r_target \/ scheduler_has_rule s2 r_target)
-        | SPos p s => scheduler_has_rule s r_target
-        end.
-    
-    Lemma scheduler_has_rule_dec:
-        forall (s: sched) (r: rule_name_t),
-        {scheduler_has_rule s r} + {~ scheduler_has_rule s r}.
-    Proof.
-        induction s; intros; simpl.
-        - right; intros H; inversion H.
-        - destruct (eq_dec r r0).
-            + left; auto.
-            + specialize (IHs r0). auto.
-        - destruct (eq_dec r r0).
-            + left; auto.
-            + specialize (IHs1 r0). specialize (IHs2 r0).
-                destruct IHs1; destruct IHs2.
-                * left; auto.
-                * left; auto.
-                * left; auto.
-                * right. intros [H1 | H2]; auto.
-        - specialize (IHs r). auto.
-    Qed.
+  Fixpoint scheduler_has_rule (scheduler : sched) (r_target : rule_name_t) : Prop :=
+    match scheduler with
+    | Done => False
+    | Cons r s => if eq_dec r r_target then True else scheduler_has_rule s r_target
+    | Try r s1 s2 => if eq_dec r r_target then True else (scheduler_has_rule s1 r_target \/ scheduler_has_rule s2 r_target)
+    | SPos p s => scheduler_has_rule s r_target
+    end.
+  
+  Lemma scheduler_has_rule_dec:
+    forall (s: sched) (r: rule_name_t),
+    {scheduler_has_rule s r} + {~ scheduler_has_rule s r}.
+  Proof.
+    induction s; intros; simpl.
+    - right; intros H; inversion H.
+    - destruct (eq_dec r r0).
+      + left; auto.
+      + specialize (IHs r0). auto.
+    - destruct (eq_dec r r0).
+      + left; auto.
+      + specialize (IHs1 r0). specialize (IHs2 r0).
+        destruct IHs1; destruct IHs2.
+        * left; auto.
+        * left; auto.
+        * left; auto.
+        * right. intros [H1 | H2]; auto.
+    - specialize (IHs r). auto.
+  Qed.
 
-    Lemma scheduler_has_not_rule_inductive:
-        forall (s: sched) (r: rule_name_t),
-        ~ scheduler_has_rule s r ->
-            match s with
-            | Done => True
-            | Cons r0 s' => if eq_dec r0 r then False else ~ scheduler_has_rule s' r
-            | Try r0 s1 s2 => if eq_dec r0 r then False else (~ scheduler_has_rule s1 r /\ ~ scheduler_has_rule s2 r)
-            | SPos p s' => ~ scheduler_has_rule s' r
-            end.
-    Proof.
-        induction s; intros; simpl in *.
-        - auto.
-        - destruct (eq_dec r r0).
-            + exfalso; apply H. (* hammer. *) sfirstorder.
-            + (* hammer. *) sfirstorder.
-        - destruct (eq_dec r r0).
-            + exfalso; apply H. (* hammer. *) sfirstorder.
-            + (* hammer. *) sfirstorder.
-        - (* hammer. *) sfirstorder.
-    Qed.
+  Lemma scheduler_has_not_rule_inductive:
+    forall (s: sched) (r: rule_name_t),
+    ~ scheduler_has_rule s r ->
+      match s with
+      | Done => True
+      | Cons r0 s' => if eq_dec r0 r then False else ~ scheduler_has_rule s' r
+      | Try r0 s1 s2 => if eq_dec r0 r then False else (~ scheduler_has_rule s1 r /\ ~ scheduler_has_rule s2 r)
+      | SPos p s' => ~ scheduler_has_rule s' r
+      end.
+  Proof.
+    induction s; intros; simpl in *.
+    - auto.
+    - destruct (eq_dec r r0).
+      + exfalso; apply H. (* hammer. *) sfirstorder.
+      + (* hammer. *) sfirstorder.
+    - destruct (eq_dec r r0).
+      + exfalso; apply H. (* hammer. *) sfirstorder.
+      + (* hammer. *) sfirstorder.
+    - (* hammer. *) sfirstorder.
+  Qed.
 
 End Schedule.
 
 Section Environments.
 
-    Lemma getenv_ccreate:
-         forall {K : Type} {FT: FiniteType K}
-            {V : esig K}
-            (fn : forall k : K, V k)
-            (k : K),
-            ContextEnv.(getenv) (ccreate finite_elements (fun k _ => fn k)) k = fn k.
-    Proof.
-        intros. unfold getenv. cbn.
-        rewrite cassoc_ccreate. reflexivity.
-    Qed.
+  Lemma getenv_ccreate:
+     forall {K : Type} {FT: FiniteType K}
+      {V : esig K}
+      (fn : forall k : K, V k)
+      (k : K),
+      ContextEnv.(getenv) (ccreate finite_elements (fun k _ => fn k)) k = fn k.
+  Proof.
+    intros. unfold getenv. cbn.
+    rewrite cassoc_ccreate. reflexivity.
+  Qed.
 
-    Lemma get_put_eq:
-        forall {K : Type} {FT: FiniteType K} {V : esig K} (ev : env_t ContextEnv V) (k : K) (v : V k),
-            ContextEnv.(getenv) (ContextEnv.(putenv) ev k v) k = v.
-    Proof.
-        intros. rewrite get_put_eq. reflexivity.
-    Qed.
+  Lemma get_put_eq:
+    forall {K : Type} {FT: FiniteType K} {V : esig K} (ev : env_t ContextEnv V) (k : K) (v : V k),
+      ContextEnv.(getenv) (ContextEnv.(putenv) ev k v) k = v.
+  Proof.
+    intros. rewrite get_put_eq. reflexivity.
+  Qed.
 
-    Lemma cassoc_put_eq:
-        forall {K : Type} {FT: FiniteType K} {V : esig K} (ev : env_t ContextEnv V) (k : K) (v : V k),
-            cassoc (finite_member k) (ContextEnv.(putenv) ev k v) = v.
-    Proof.
-        intros. generalize (get_put_eq ev k v). intros H.
-        unfold getenv in H. cbn in *. rewrite H. reflexivity.
-    Qed.
+  Lemma cassoc_put_eq:
+    forall {K : Type} {FT: FiniteType K} {V : esig K} (ev : env_t ContextEnv V) (k : K) (v : V k),
+      cassoc (finite_member k) (ContextEnv.(putenv) ev k v) = v.
+  Proof.
+    intros. generalize (get_put_eq ev k v). intros H.
+    unfold getenv in H. cbn in *. rewrite H. reflexivity.
+  Qed.
 
-    Lemma get_put_neq:
-        forall {K : Type} {FT: FiniteType K} {V : esig K} (ev : env_t ContextEnv V) (k k' : K) (v : V k),
-            k <> k' ->
-            ContextEnv.(getenv) (ContextEnv.(putenv) ev k v) k' = ContextEnv.(getenv) ev k'.
-    Proof.
-        intros. rewrite get_put_neq. reflexivity. sfirstorder.
-    Qed.
+  Lemma get_put_neq:
+    forall {K : Type} {FT: FiniteType K} {V : esig K} (ev : env_t ContextEnv V) (k k' : K) (v : V k),
+      k <> k' ->
+      ContextEnv.(getenv) (ContextEnv.(putenv) ev k v) k' = ContextEnv.(getenv) ev k'.
+  Proof.
+    intros. rewrite get_put_neq. reflexivity. sfirstorder.
+  Qed.
 
-    Lemma cassoc_put_neq:
-        forall {K : Type} {FT: FiniteType K} {V : esig K} (ev : env_t ContextEnv V) (k k' : K) (v : V k),
-            k <> k' ->
-            cassoc (finite_member k') (ContextEnv.(putenv) ev k v) = cassoc (finite_member k') ev.
-    Proof.
-        intros. generalize (get_put_neq ev k k' v H). intros Hget.
-        unfold getenv in Hget. cbn in *. rewrite Hget. reflexivity.
-    Qed.
+  Lemma cassoc_put_neq:
+    forall {K : Type} {FT: FiniteType K} {V : esig K} (ev : env_t ContextEnv V) (k k' : K) (v : V k),
+      k <> k' ->
+      cassoc (finite_member k') (ContextEnv.(putenv) ev k v) = cassoc (finite_member k') ev.
+  Proof.
+    intros. generalize (get_put_neq ev k k' v H). intros Hget.
+    unfold getenv in Hget. cbn in *. rewrite Hget. reflexivity.
+  Qed.
 
 End Environments.
 
 Section BitsToLists.
-    
-    Lemma bits_to_list_assoc_fallback_cons:
-        forall {K V: Type} {eq: EqDec K} (l: list (K * V)) (k: K) x k1 v1,
-        BitsToLists.list_assoc l k = Some x -> 
-            BitsToLists.list_assoc ((k1, v1) :: l) k <> None.
-    Proof.
-        intros. unfold not. intros.  unfold BitsToLists.list_assoc in *. 
-        destruct (eq_dec k k1).
-        - inversion H0.
-        - hauto.
-    Qed.
-    
-    Lemma bits_to_list_assoc_fallback_app:
-        forall {K V: Type} {eq: EqDec K} (l: list (K * V)) (k: K) x a,
-        BitsToLists.list_assoc l k = Some x -> 
-            BitsToLists.list_assoc (a ++ l) k <> None.
-    Proof.
-        intros. unfold not. intros. unfold BitsToLists.list_assoc in *.
-        generalize dependent H.
-        induction a; intros. 
-        { rewrite app_nil_l in H0. (* hammer. *) timeout 10 sfirstorder. }
-        rewrite <- app_comm_cons in H0.
-        cbn in H0. destruct a as [k1 v1].
-        destruct (eq_dec k k1).
-        - inversion H0.
-        - hauto.
-    Qed.
+  
+  Lemma bits_to_list_assoc_fallback_cons:
+    forall {K V: Type} {eq: EqDec K} (l: list (K * V)) (k: K) x k1 v1,
+    BitsToLists.list_assoc l k = Some x -> 
+      BitsToLists.list_assoc ((k1, v1) :: l) k <> None.
+  Proof.
+    intros. unfold not. intros.  unfold BitsToLists.list_assoc in *. 
+    destruct (eq_dec k k1).
+    - inversion H0.
+    - hauto.
+  Qed.
+  
+  Lemma bits_to_list_assoc_fallback_app:
+    forall {K V: Type} {eq: EqDec K} (l: list (K * V)) (k: K) x a,
+    BitsToLists.list_assoc l k = Some x -> 
+      BitsToLists.list_assoc (a ++ l) k <> None.
+  Proof.
+    intros. unfold not. intros. unfold BitsToLists.list_assoc in *.
+    generalize dependent H.
+    induction a; intros. 
+    { rewrite app_nil_l in H0. (* hammer. *) timeout 10 sfirstorder. }
+    rewrite <- app_comm_cons in H0.
+    cbn in H0. destruct a as [k1 v1].
+    destruct (eq_dec k k1).
+    - inversion H0.
+    - hauto.
+  Qed.
 
-    Lemma bits_to_list_assoc_app:
-        forall {K V: Type} {eq: EqDec K} (l: list (K * V)) (k: K) x a,
-        BitsToLists.list_assoc l k = Some x -> 
-            BitsToLists.list_assoc (l ++ a) k = Some x.
-    Proof.
-        intros. generalize dependent H.
-        induction l; intros; cbn in *; try congruence.
-        destruct a0 as [k1 v1]. destruct (eq_dec k k1).
-        - subst. exact H.
-        - apply IHl. exact H.
-    Qed.
+  Lemma bits_to_list_assoc_app:
+    forall {K V: Type} {eq: EqDec K} (l: list (K * V)) (k: K) x a,
+    BitsToLists.list_assoc l k = Some x -> 
+      BitsToLists.list_assoc (l ++ a) k = Some x.
+  Proof.
+    intros. generalize dependent H.
+    induction l; intros; cbn in *; try congruence.
+    destruct a0 as [k1 v1]. destruct (eq_dec k k1).
+    - subst. exact H.
+    - apply IHl. exact H.
+  Qed.
 
-    Lemma bits_to_list_assoc_app_not_in:
-        forall {K V: Type} {eq: EqDec K} (l: list (K * V)) (k: K) x a,
-        ~ In k (map fst a) ->
-        BitsToLists.list_assoc l k = Some x -> 
-            BitsToLists.list_assoc (a ++ l) k = Some x.
-    Proof.
-        intros. generalize dependent H0.
-        induction a; intros; cbn in *.
-        - exact H0.
-        - destruct a as [k1 v1]. destruct (eq_dec k k1).
-            + subst. contradict H. left. reflexivity.
-            + apply IHa; auto.
-    Qed.
+  Lemma bits_to_list_assoc_app_not_in:
+    forall {K V: Type} {eq: EqDec K} (l: list (K * V)) (k: K) x a,
+    ~ In k (map fst a) ->
+    BitsToLists.list_assoc l k = Some x -> 
+      BitsToLists.list_assoc (a ++ l) k = Some x.
+  Proof.
+    intros. generalize dependent H0.
+    induction a; intros; cbn in *.
+    - exact H0.
+    - destruct a as [k1 v1]. destruct (eq_dec k k1).
+      + subst. contradict H. left. reflexivity.
+      + apply IHa; auto.
+  Qed.
 
-    Lemma bits_to_list_assoc_app_not_in2:
-        forall {K V: Type} {eq: EqDec K} (l: list (K * V)) (k: K) x a,
-        ~ In k (map fst a) ->
-        BitsToLists.list_assoc (a ++ l) k = Some x -> 
-            BitsToLists.list_assoc l k = Some x.
-    Proof.
-        intros. generalize dependent H0.
-        induction a; intros; cbn in *.
-        - exact H0.
-        - destruct a as [k1 v1]. destruct (eq_dec k k1).
-            + subst. contradict H. left. reflexivity.
-            + apply IHa; auto.
-    Qed.
+  Lemma bits_to_list_assoc_app_not_in2:
+    forall {K V: Type} {eq: EqDec K} (l: list (K * V)) (k: K) x a,
+    ~ In k (map fst a) ->
+    BitsToLists.list_assoc (a ++ l) k = Some x -> 
+      BitsToLists.list_assoc l k = Some x.
+  Proof.
+    intros. generalize dependent H0.
+    induction a; intros; cbn in *.
+    - exact H0.
+    - destruct a as [k1 v1]. destruct (eq_dec k k1).
+      + subst. contradict H. left. reflexivity.
+      + apply IHa; auto.
+  Qed.
 
-    Lemma bits_to_list_assoc_app_not_in3:
-        forall {K V: Type} {eq: EqDec K} (l: list (K * V)) (k: K) a,
-        ~ In k (map fst a) ->
-        BitsToLists.list_assoc (a ++ l) k = BitsToLists.list_assoc l k.
-    Proof.
-        intros.
-        induction a; intros; cbn in *.
-        - reflexivity.
-        - destruct a as [k1 v1]. destruct (eq_dec k k1).
-            + subst. contradict H. left. reflexivity.
-            + apply IHa; auto.
-    Qed.
+  Lemma bits_to_list_assoc_app_not_in3:
+    forall {K V: Type} {eq: EqDec K} (l: list (K * V)) (k: K) a,
+    ~ In k (map fst a) ->
+    BitsToLists.list_assoc (a ++ l) k = BitsToLists.list_assoc l k.
+  Proof.
+    intros.
+    induction a; intros; cbn in *.
+    - reflexivity.
+    - destruct a as [k1 v1]. destruct (eq_dec k k1).
+      + subst. contradict H. left. reflexivity.
+      + apply IHa; auto.
+  Qed.
 
-    Lemma bits_to_list_assoc_app_in:
-        forall {K V: Type} {eq: EqDec K} (l: list (K * V)) (k: K) a,
-        In k (map fst a) ->
-        BitsToLists.list_assoc (a ++ l) k = BitsToLists.list_assoc a k.
-    Proof.
-        intros.
-        induction a; intros; cbn in *.
-        - contradict H.
-        - destruct a as [k1 v1]. destruct (eq_dec k k1).
-            + reflexivity.
-            + destruct H.
-              * subst. cbn in n. congruence.
-              * apply IHa; auto.
-    Qed.
+  Lemma bits_to_list_assoc_app_in:
+    forall {K V: Type} {eq: EqDec K} (l: list (K * V)) (k: K) a,
+    In k (map fst a) ->
+    BitsToLists.list_assoc (a ++ l) k = BitsToLists.list_assoc a k.
+  Proof.
+    intros.
+    induction a; intros; cbn in *.
+    - contradict H.
+    - destruct a as [k1 v1]. destruct (eq_dec k k1).
+      + reflexivity.
+      + destruct H.
+        * subst. cbn in n. congruence.
+        * apply IHa; auto.
+  Qed.
 
-    Lemma bits_to_list_assoc_app3:
-        forall {K V: Type} {eq: EqDec K} (l: list (K * V)) (k: K) a,
-        ListDec.decidable_eq K ->
-        BitsToLists.list_assoc (a ++ a ++ l) k = BitsToLists.list_assoc (a ++ l) k.
-    Proof.
-        intros.
-        induction a; intros; cbn in *.
-        - reflexivity.
-        - destruct a as [k1 v1]. destruct (eq_dec k k1).
-            + reflexivity.
-            + destruct (ListDec.In_decidable H k (map fst a0)).
-              * rewrite !bits_to_list_assoc_app_in with (1:=H0). reflexivity.
-              * rewrite bits_to_list_assoc_app_not_in3 with (1:=H0). cbn. destruct (eq_dec k k1).
-                congruence. reflexivity.
-    Qed.
+  Lemma bits_to_list_assoc_app3:
+    forall {K V: Type} {eq: EqDec K} (l: list (K * V)) (k: K) a,
+    ListDec.decidable_eq K ->
+    BitsToLists.list_assoc (a ++ a ++ l) k = BitsToLists.list_assoc (a ++ l) k.
+  Proof.
+    intros.
+    induction a; intros; cbn in *.
+    - reflexivity.
+    - destruct a as [k1 v1]. destruct (eq_dec k k1).
+      + reflexivity.
+      + destruct (ListDec.In_decidable H k (map fst a0)).
+        * rewrite !bits_to_list_assoc_app_in with (1:=H0). reflexivity.
+        * rewrite bits_to_list_assoc_app_not_in3 with (1:=H0). cbn. destruct (eq_dec k k1).
+        congruence. reflexivity.
+  Qed.
 
-    Lemma bits_to_list_assoc_app_both_none:
-        forall {K V: Type} {eq: EqDec K} (l: list (K * V)) (k: K) a,
-        BitsToLists.list_assoc l k = None ->
-        BitsToLists.list_assoc a k = None -> 
-            BitsToLists.list_assoc (a ++ l) k = None.
-    Proof.
-        intros. generalize dependent H0.
-        induction a; intros; cbn in *.
-        - exact H.
-        - destruct a as [k1 v1]. destruct (eq_dec k k1).
-            + inversion H0.
-            + apply IHa; auto.
-    Qed.
+  Lemma bits_to_list_assoc_app_both_none:
+    forall {K V: Type} {eq: EqDec K} (l: list (K * V)) (k: K) a,
+    BitsToLists.list_assoc l k = None ->
+    BitsToLists.list_assoc a k = None -> 
+      BitsToLists.list_assoc (a ++ l) k = None.
+  Proof.
+    intros. generalize dependent H0.
+    induction a; intros; cbn in *.
+    - exact H.
+    - destruct a as [k1 v1]. destruct (eq_dec k k1).
+      + inversion H0.
+      + apply IHa; auto.
+  Qed.
 
-    Lemma bits_to_list_assoc_app_both_none1:
-        forall {K V: Type} {eq: EqDec K} (l: list (K * V)) (k: K) a,
-        BitsToLists.list_assoc a k = None -> 
-            BitsToLists.list_assoc (a ++ l) k = BitsToLists.list_assoc l k.
-    Proof.
-        intros. generalize dependent H.
-        induction a; intros; cbn in *.
-        - reflexivity.
-        - destruct a as [k1 v1]. destruct (eq_dec k k1).
-            + inversion H.
-            + apply IHa; auto.
-    Qed.
+  Lemma bits_to_list_assoc_app_both_none1:
+    forall {K V: Type} {eq: EqDec K} (l: list (K * V)) (k: K) a,
+    BitsToLists.list_assoc a k = None -> 
+      BitsToLists.list_assoc (a ++ l) k = BitsToLists.list_assoc l k.
+  Proof.
+    intros. generalize dependent H.
+    induction a; intros; cbn in *.
+    - reflexivity.
+    - destruct a as [k1 v1]. destruct (eq_dec k k1).
+      + inversion H.
+      + apply IHa; auto.
+  Qed.
 
-    Lemma bits_to_list_assoc_app_not_in_middle:
-        forall {K V: Type} {eq: EqDec K} (l1 l2: list (K * V)) (k: K) a,
-        ~ In k (map fst a) ->
-        BitsToLists.list_assoc (l1 ++ a ++ l2) k = BitsToLists.list_assoc (l1 ++ l2) k.
-    Proof.
-        intros.
-        induction a; intros; cbn in *.
-        - reflexivity.
-        - destruct a as [k1 v1]. destruct (eq_dec k k1).
-          + subst. contradict H. left. reflexivity.
-          + destruct (BitsToLists.list_assoc l1 k) eqn:Hassoc.
-            * rewrite !bits_to_list_assoc_app with (x:=v) (1:=Hassoc). reflexivity.
-            * rewrite !bits_to_list_assoc_app_both_none1 with (1:=Hassoc) in *. cbn. destruct (eq_dec k k1); try congruence.
-              apply IHa. intro; apply H. right. exact H0.
-    Qed.
+  Lemma bits_to_list_assoc_app_not_in_middle:
+    forall {K V: Type} {eq: EqDec K} (l1 l2: list (K * V)) (k: K) a,
+    ~ In k (map fst a) ->
+    BitsToLists.list_assoc (l1 ++ a ++ l2) k = BitsToLists.list_assoc (l1 ++ l2) k.
+  Proof.
+    intros.
+    induction a; intros; cbn in *.
+    - reflexivity.
+    - destruct a as [k1 v1]. destruct (eq_dec k k1).
+      + subst. contradict H. left. reflexivity.
+      + destruct (BitsToLists.list_assoc l1 k) eqn:Hassoc.
+      * rewrite !bits_to_list_assoc_app with (x:=v) (1:=Hassoc). reflexivity.
+      * rewrite !bits_to_list_assoc_app_both_none1 with (1:=Hassoc) in *. cbn. destruct (eq_dec k k1); try congruence.
+        apply IHa. intro; apply H. right. exact H0.
+  Qed.
 
-    Lemma bits_of_list_vect_to_list:
-        forall {n} (b: bits n),
-            Bits.of_list (vect_to_list b) = rew [vect bool] (BitsToLists.len_to_list n b) in b.
-    Proof.
-        intros. apply vect_to_list_inj. rewrite BitsToLists.vect_to_list_of_list.
-        rewrite vect_to_list_eq_rect. reflexivity.
-    Qed. 
-    
-    Lemma vect_fold_left_of_zeros:
-        forall n acc,
-            vect_fold_left (fun (acc : list bool) (t : bool) => t :: acc) acc (Bits.zeroes n) = repeat false n ++ acc.
-    Proof.
-        intros. induction n; intros; simpl. reflexivity.
-        rewrite IHn. simpl. reflexivity.
-    Qed.
+  Lemma bits_of_list_vect_to_list:
+    forall {n} (b: bits n),
+      Bits.of_list (vect_to_list b) = rew [vect bool] (BitsToLists.len_to_list n b) in b.
+  Proof.
+    intros. apply vect_to_list_inj. rewrite BitsToLists.vect_to_list_of_list.
+    rewrite vect_to_list_eq_rect. reflexivity.
+  Qed. 
+  
+  Lemma vect_fold_left_of_zeros:
+    forall n acc,
+      vect_fold_left (fun (acc : list bool) (t : bool) => t :: acc) acc (Bits.zeroes n) = repeat false n ++ acc.
+  Proof.
+    intros. induction n; intros; simpl. reflexivity.
+    rewrite IHn. simpl. reflexivity.
+  Qed.
 
 End BitsToLists.
 
 Section ContextLogs.
-    Context {V: Type}.
+  Context {V: Type}.
 
-    Context {reg_t: Type}.
-    Context {reg_t_finite : FiniteType reg_t}.
+  Context {reg_t: Type}.
+  Context {reg_t_finite : FiniteType reg_t}.
 
-    Notation CEnv := (@ContextEnv reg_t reg_t_finite).
-    Notation Log := (@_ULog V reg_t CEnv).
+  Notation CEnv := (@ContextEnv reg_t reg_t_finite).
+  Notation Log := (@_ULog V reg_t CEnv).
 
-    Lemma log_existsb_context_concat:
-        forall (logX logY : Log) (elemX : reg_t) (c : env_t ContextEnv (fun _ : reg_t => list (LogEntry V))) isX,
-            log_existsb logX elemX isX = log_existsb logY elemX isX ->
-            @log_existsb V reg_t CEnv (ccreate finite_elements (fun (k : reg_t) (_ : member k finite_elements) => c.[k] ++ logX.[k])) elemX isX =
-            @log_existsb V reg_t CEnv (ccreate finite_elements (fun (k : reg_t) (_ : member k finite_elements) => c.[k] ++ logY.[k])) elemX isX.
-    Proof.
-        intros. unfold log_existsb in *. rewrite !getenv_ccreate.
-        rewrite !existsb_app. rewrite H. reflexivity.
-    Qed.
+  Lemma ulog_existsb_context_concat:
+    forall (logX logY : Log) (elemX : reg_t) (c : env_t ContextEnv (fun _ : reg_t => list (LogEntry V))) isX,
+      log_existsb logX elemX isX = log_existsb logY elemX isX ->
+      @log_existsb V reg_t CEnv (ccreate finite_elements (fun (k : reg_t) (_ : member k finite_elements) => c.[k] ++ logX.[k])) elemX isX =
+      @log_existsb V reg_t CEnv (ccreate finite_elements (fun (k : reg_t) (_ : member k finite_elements) => c.[k] ++ logY.[k])) elemX isX.
+  Proof.
+    intros. unfold log_existsb in *. rewrite !getenv_ccreate.
+    rewrite !existsb_app. rewrite H. reflexivity.
+  Qed.
 
-    Lemma cassoc_log_cons_neq:
-        forall (log: Log) (idx idx': reg_t) (le: LogEntry V),
-            idx <> idx' ->
-            cassoc (finite_member idx') (log_cons idx le log) = cassoc (finite_member idx') log.
-    Proof.
-        intros. unfold log_cons. rewrite cassoc_put_neq. 2: exact H. reflexivity.
-    Qed.
+  Lemma cassoc_log_cons_neq:
+    forall (log: Log) (idx idx': reg_t) (le: LogEntry V),
+      idx <> idx' ->
+      cassoc (finite_member idx') (log_cons idx le log) = cassoc (finite_member idx') log.
+  Proof.
+    intros. unfold log_cons. rewrite cassoc_put_neq. 2: exact H. reflexivity.
+  Qed.
 
-    Lemma cassoc_log_cons_eq:
-        forall (log: Log) (idx: reg_t) (le: LogEntry V),
-            cassoc (finite_member idx) (log_cons idx le log) = le :: cassoc (finite_member idx) log.
-    Proof.
-        intros. unfold log_cons. rewrite cassoc_put_eq. reflexivity.
-    Qed.
+  Lemma cassoc_log_cons_eq:
+    forall (log: Log) (idx: reg_t) (le: LogEntry V),
+      cassoc (finite_member idx) (log_cons idx le log) = le :: cassoc (finite_member idx) log.
+  Proof.
+    intros. unfold log_cons. rewrite cassoc_put_eq. reflexivity.
+  Qed.
 
-    Lemma cassoc_log_app:
-        forall (log1 log2: Log) (idx: reg_t),
-            cassoc (finite_member idx) (log_app log1 log2) = cassoc (finite_member idx) log1 ++ cassoc (finite_member idx) log2.
-    Proof.
-        intros. unfold log_app. simpl. rewrite cassoc_ccreate. unfold getenv. cbn. reflexivity.
-    Qed.
+  Lemma cassoc_log_app:
+    forall (log1 log2: Log) (idx: reg_t),
+      cassoc (finite_member idx) (log_app log1 log2) = cassoc (finite_member idx) log1 ++ cassoc (finite_member idx) log2.
+  Proof.
+    intros. unfold log_app. simpl. rewrite cassoc_ccreate. unfold getenv. cbn. reflexivity.
+  Qed.
 
 End ContextLogs.
 
 Section Datatypes.
 
-    Lemma datatypes_length_vect_fold_left_of_bits:
-        forall {n} (v : bits n),
-            Datatypes.length (vect_fold_left (fun (acc : list bool) (t : bool) => t :: acc) [] v) = n.
-    Proof.
-        intros. unfold vect_fold_left.
-        induction n; intros; simpl. reflexivity.
-        rewrite IHn. simpl. lia.
-    Qed.
+  Lemma datatypes_length_vect_fold_left_of_bits:
+    forall {n} (v : bits n),
+      Datatypes.length (vect_fold_left (fun (acc : list bool) (t : bool) => t :: acc) [] v) = n.
+  Proof.
+    intros. unfold vect_fold_left.
+    induction n; intros; simpl. reflexivity.
+    rewrite IHn. simpl. lia.
+  Qed.
 
-    Lemma datatypes_length_firstn_vect_fold_left_of_bits':
-        forall {n} (v : bits n),
-            Datatypes.length (firstn n (vect_fold_left (fun (acc : list bool) (t : bool) => t :: acc) [] v)) = n.
-    Proof.
-        intros. unfold vect_fold_left.
-        induction n; intros; simpl. reflexivity.
-        rewrite IHn. simpl. lia.
-    Qed.
+  Lemma datatypes_length_firstn_vect_fold_left_of_bits':
+    forall {n} (v : bits n),
+      Datatypes.length (firstn n (vect_fold_left (fun (acc : list bool) (t : bool) => t :: acc) [] v)) = n.
+  Proof.
+    intros. unfold vect_fold_left.
+    induction n; intros; simpl. reflexivity.
+    rewrite IHn. simpl. lia.
+  Qed.
 
-    Lemma datatypes_length_firstn_vect_fold_left_of_bits:
-        forall {n} x (v : bits n),
-            x < n ->
-            Datatypes.length (firstn x (vect_fold_left (fun (acc : list bool) (t : bool) => t :: acc) [] v)) = x.
-    Proof.
-        unfold vect_fold_left.
-        induction n; intros; simpl. lia.
-        destruct x; simpl. reflexivity.
-        rewrite IHn; lia.
-    Qed.
+  Lemma datatypes_length_firstn_vect_fold_left_of_bits:
+    forall {n} x (v : bits n),
+      x < n ->
+      Datatypes.length (firstn x (vect_fold_left (fun (acc : list bool) (t : bool) => t :: acc) [] v)) = x.
+  Proof.
+    unfold vect_fold_left.
+    induction n; intros; simpl. lia.
+    destruct x; simpl. reflexivity.
+    rewrite IHn; lia.
+  Qed.
 
-    Lemma repeat_nil:
-        forall {A: Type} n (a: A),
-        n = 0%nat ->
-        repeat a n = [].
-    Proof.
-        intros. subst. reflexivity.
-    Qed.
+  Lemma repeat_nil:
+    forall {A: Type} n (a: A),
+    n = 0%nat ->
+    repeat a n = [].
+  Proof.
+    intros. subst. reflexivity.
+  Qed.
 
-    Lemma datatypes_length_bitwise:
-        forall l1 l2 f,
-            Datatypes.length (BitsToLists.bitwise f l1 l2) = Nat.max (Datatypes.length l1) (Datatypes.length l2).
-    Proof.
-        intros. 
-        generalize dependent l2.
-        induction l1; intros.
-        - cbn. destruct l2; simpl. reflexivity. 
-          rewrite map_length. reflexivity.
-        - cbn. destruct l2.
-          + cbn. rewrite map_length. reflexivity.
-          + cbn. rewrite IHl1. reflexivity.
-    Qed.
+  Lemma datatypes_length_bitwise:
+    forall l1 l2 f,
+      Datatypes.length (BitsToLists.bitwise f l1 l2) = Nat.max (Datatypes.length l1) (Datatypes.length l2).
+  Proof.
+    intros. 
+    generalize dependent l2.
+    induction l1; intros.
+    - cbn. destruct l2; simpl. reflexivity. 
+      rewrite map_length. reflexivity.
+    - cbn. destruct l2.
+      + cbn. rewrite map_length. reflexivity.
+      + cbn. rewrite IHl1. reflexivity.
+  Qed.
 
 End Datatypes.
 
 Section Lists.
 
-    Lemma in_filter_means_in_filter_cons:
-        forall {A: Type} (f: A -> bool) (l: list A) a b,
-        In a (filter f l) ->
-        In a (filter f (b :: l)).
-    Proof.
-        intros. destruct (f b) eqn:Hfb; cbn; rewrite Hfb.
-        - right. exact H.
-        - exact H.
-    Qed.
+  Lemma in_filter_means_in_filter_cons:
+    forall {A: Type} (f: A -> bool) (l: list A) a b,
+    In a (filter f l) ->
+    In a (filter f (b :: l)).
+  Proof.
+    intros. destruct (f b) eqn:Hfb; cbn; rewrite Hfb.
+    - right. exact H.
+    - exact H.
+  Qed.
 
 End Lists.
 
 Section Bits.
 
-    Lemma bits_single_is_neg_beq_dec:
-        forall x, beq_dec x Ob~0 = negb (Bits.single x).
-    Proof.
-        intros. unfold Bits.single, beq_dec.
-        destruct x. destruct vtl. destruct vhd; cbn; auto.
-    Qed. 
+  Lemma bits_single_is_neg_beq_dec:
+    forall x, beq_dec x Ob~0 = negb (Bits.single x).
+  Proof.
+    intros. unfold Bits.single, beq_dec.
+    destruct x. destruct vtl. destruct vhd; cbn; auto.
+  Qed. 
 
 End Bits.
 
 Section Helper.
 
-    Lemma tl_skipn:
-        forall {T} (l: list T) n,
-        tl (List.skipn n l) = List.skipn (S n) l.
-    Proof.
-        intros.
-        generalize dependent l.
-        induction n; intros; simpl.
-        - reflexivity.
-        - destruct l; simpl in *; try reflexivity. apply IHn.
-    Qed.
+  Lemma tl_skipn:
+    forall {T} (l: list T) n,
+    tl (List.skipn n l) = List.skipn (S n) l.
+  Proof.
+    intros.
+    generalize dependent l.
+    induction n; intros; simpl.
+    - reflexivity.
+    - destruct l; simpl in *; try reflexivity. apply IHn.
+    Show Proof.
+  Qed.
 
-    Lemma pair_inj':
-        forall {A B: Type} (p1 p2: A * B),
-        fst p1 = fst p2 ->
-        snd p1 = snd p2 ->
-        p1 = p2.
-    Proof.
-        intros. destruct p1. destruct p2. simpl in *.
-        subst. reflexivity.
-    Qed.
+  Lemma pair_inj':
+    forall {A B: Type} (p1 p2: A * B),
+    fst p1 = fst p2 ->
+    snd p1 = snd p2 ->
+    p1 = p2.
+  Proof.
+    intros. destruct p1. destruct p2. simpl in *.
+    subst. reflexivity.
+  Qed.
 
-    Lemma tf_h_match_skipn_cons:
-        forall {T1 T2 T3} (X1 X2: option (T1 * T2 * list T3)) n1 n2,
-        n2 = S n1 ->
-        X1 = X2 ->
-        match
-            match X1 with
-            | Some (l, v, G) => Some (l, v, List.skipn n1 G)
-            | None => None
-            end
-        with
-        | Some (l, v, G) => Some (l, v, tl G)
-        | None => None
-        end = match X2 with
-        | Some (l, v, G) => Some (l, v, List.skipn n2 G)
-        | None => None
-        end.
-    Proof.
-        intros. rewrite H, H0. destruct X2 as [[[l v] G]|]; simpl.
-        - repeat f_equal. destruct G.
-          * rewrite skipn_nil. reflexivity.
-          * rewrite tl_skipn. reflexivity.
-        - reflexivity.
-    Qed.
+  Lemma tf_h_match_skipn_cons:
+    forall {T1 T2 T3} (X1 X2: option (T1 * T2 * list T3)) n1 n2,
+    n2 = S n1 ->
+    X1 = X2 ->
+    match
+      match X1 with
+      | Some (l, v, G) => Some (l, v, List.skipn n1 G)
+      | None => None
+      end
+    with
+    | Some (l, v, G) => Some (l, v, tl G)
+    | None => None
+    end = match X2 with
+    | Some (l, v, G) => Some (l, v, List.skipn n2 G)
+    | None => None
+    end.
+  Proof.
+    intros. rewrite H, H0. destruct X2 as [[[l v] G]|]; simpl.
+    - repeat f_equal. destruct G.
+      * rewrite skipn_nil. reflexivity.
+      * rewrite tl_skipn. reflexivity.
+    - reflexivity.
+  Qed.
 
-    Lemma tf_h_match_skipn:
-        forall {T1 T2 T3} (X1 X2: option (T1 * T2 * list T3)) n1 n2,
-        n2 = n1 ->
-        X1 = X2 ->
-        match X1 with
-        | Some (l, v, G) => Some (l, v, List.skipn n1 G)
-        | None => None
-        end = match X2 with
-        | Some (l, v, G) => Some (l, v, List.skipn n2 G)
-        | None => None
-        end.
-    Proof.
-        intros. rewrite H, H0. destruct X2 as [[[l v] G]|]; simpl; reflexivity.
-    Qed.
+  Lemma tf_h_match_skipn:
+    forall {T1 T2 T3} (X1 X2: option (T1 * T2 * list T3)) n1 n2,
+    n2 = n1 ->
+    X1 = X2 ->
+    match X1 with
+    | Some (l, v, G) => Some (l, v, List.skipn n1 G)
+    | None => None
+    end = match X2 with
+    | Some (l, v, G) => Some (l, v, List.skipn n2 G)
+    | None => None
+    end.
+  Proof.
+    intros. rewrite H, H0. destruct X2 as [[[l v] G]|]; simpl; reflexivity.
+  Qed.
 
-    Lemma tf_h_match_skipn_app:
-        forall {T1 T2 T3} (X1 X2: option (T1 * T2 * list T3)) n1 n2 n3,
-        n3 = n1 + n2 ->
-        X1 = X2 ->
-        match
-            match X1 with
-            | Some (l, v, G) => Some (l, v, List.skipn n1 G)
-            | None => None
-            end
-        with
-        | Some (l, v, G) => Some (l, v, List.skipn n2 G)
-        | None => None
-        end = match X2 with
-        | Some (l, v, G) => Some (l, v, List.skipn n3 G)
-        | None => None
-        end.
-    Proof.
-        intros. rewrite H, H0. destruct X2 as [[[l v] G]|]; simpl.
-        - f_equal. f_equal. clear H H0. generalize dependent G.
-            induction n1 as [| n1' IH]; intros.
-            + reflexivity.
-            + cbn. destruct G.
-              * rewrite skipn_nil. reflexivity.
-              * apply IH.
-        - reflexivity.
-    Qed.
-        
+  Lemma tf_h_match_skipn_app:
+    forall {T1 T2 T3} (X1 X2: option (T1 * T2 * list T3)) n1 n2 n3,
+    n3 = n1 + n2 ->
+    X1 = X2 ->
+    match
+      match X1 with
+      | Some (l, v, G) => Some (l, v, List.skipn n1 G)
+      | None => None
+      end
+    with
+    | Some (l, v, G) => Some (l, v, List.skipn n2 G)
+    | None => None
+    end = match X2 with
+    | Some (l, v, G) => Some (l, v, List.skipn n3 G)
+    | None => None
+    end.
+  Proof.
+    intros. rewrite H, H0. destruct X2 as [[[l v] G]|]; simpl.
+    - f_equal. f_equal. clear H H0. generalize dependent G.
+      induction n1 as [| n1' IH]; intros.
+      + reflexivity.
+      + cbn. destruct G.
+        * rewrite skipn_nil. reflexivity.
+        * apply IH.
+    - reflexivity.
+  Qed.
+    
 
 End Helper.
 
+Require Import Koika.KoikaForm.Logs.
+Require Koika.Properties.SemanticProperties.
 
+Section LogHelpers.
+
+  Context {reg_t: Type}.
+  Context {reg_t_eq_dec: EqDec reg_t}.
+  Context {R: reg_t -> type}.
+  Context {REnv: Env reg_t}.
+
+  (** Lemma for searching a newly added entry (log_cons) **)
+  Lemma log_existsb_cons : forall (l : Log R REnv) (idx : reg_t) (entry : LogEntry (R idx)) (r : reg_t) (f : LogEntryKind -> Port -> bool),
+    log_existsb (log_cons idx entry l) r f = 
+    ((if eq_dec idx r then f (kind entry) (port entry) else false) || log_existsb l r f).
+  Proof.
+    intros. unfold log_existsb, log_cons.
+    destruct (eq_dec idx r).
+    - subst r. rewrite (get_put_eq REnv).
+      simpl. destruct entry. reflexivity.
+    - rewrite (get_put_neq REnv); auto.
+  Qed.
+
+  (** Lemma for searching an empty log **)
+  Lemma log_existsb_empty : forall (r : reg_t) (f : LogEntryKind -> Port -> bool),
+    log_existsb (REnv:=REnv) (R:=R) log_empty r f = false.
+  Proof.
+    (* log_empty is defined as an environment of empty lists. *)
+    intros. unfold log_existsb, log_empty.
+    rewrite getenv_create. reflexivity.
+  Qed.
+
+  Lemma may_write_log_combine :
+    forall log1 log2 P idx, 
+      may_write (reg_t:=reg_t) (R:=R) (REnv:=REnv) log1 log2 P idx = 
+      may_write (reg_t:=reg_t) (R:=R) (REnv:=REnv) (log_app log2 log1) log_empty P idx.
+  Proof.
+    intros. unfold may_write. rewrite !SemanticProperties.log_app_empty_r.
+    reflexivity.
+  Qed.
+
+  (* Lemma may_write_log_cons :
+    forall log1 log2 idx idx' le P,
+      may_write (reg_t:=reg_t) (R:=R) (REnv:=REnv) log1 (log_cons idx' le log2) P idx = 
+      (if eq_dec idx' idx then 
+        (if P =? P0 && is_write0 (kind le) (port le) then
+          false
+        else
+          may_write log1 log2 P idx) 
+      else 
+        may_write log1 log2 P idx).
+  Proof.
+    intros. unfold may_write. rewrite !SemanticProperties.log_existsb_app.
+    destruct (eq_dec idx' idx); simpl.
+    - subst idx. destruct (is_write0 (kind le) (port le)) eqn:His.
+      + rewrite !log_existsb_cons. rewrite !eq_dec_refl. rewrite !His. bool_step.
+       simpl. reflexivity.
+    - simpl. rewrite log_existsb_empty. reflexivity.
+  Qed. *)
+
+  Lemma latest_write_log_cons_read :
+    forall log idx idx' le,
+      kind le = LogRead ->
+      latest_write (reg_t:=reg_t) (R:=R) (REnv:=REnv) (log_cons idx' le log) idx = latest_write (reg_t:=reg_t) (R:=R) (REnv:=REnv) log idx.
+  Proof.
+    intros. unfold latest_write.
+    destruct (eq_dec idx' idx).
+    - subst idx'. rewrite SemanticProperties.log_find_cons_eq. destruct le; simpl; auto. destruct kind; simpl; auto.
+      contradict H. sauto.
+    - rewrite SemanticProperties.log_find_cons_neq; auto.
+  Qed.
+
+End LogHelpers.
+
+Section ListHelpers.
+
+  Context {A: Type}.
+  Context {A_eq_dec: EqDec A}.
+  Context {B: Type}.
+  Context {B_eq_dec: EqDec B}.
+
+  Lemma in_dec (x: A) (l: list A): {In x l} + {~ In x l}.
+  Proof.
+    intros. induction l.
+    - right. intros H. inversion H.
+    - destruct (eq_dec x a).
+      + left. subst. left. reflexivity.
+      + specialize (IHl). destruct IHl.
+        * left. right. exact i.
+        * right. intros H. destruct H.
+          { subst. contradiction. }
+          { apply n0. exact H. }
+  Qed.
+
+  Lemma not_in_map :
+    forall (f: A -> B) x l,
+    ~ In x l ->
+    (forall y1 y2, f y1 = f y2 -> y1 = y2) ->
+    ~ In (f x) (map f l).
+  Proof.
+    intros. intros HL. apply in_map_iff in HL. destruct HL as [y [Hfy Hin]]. 
+    specialize (H0 y x Hfy). subst. congruence.
+  Qed.
+
+End ListHelpers.
+
+Section MatchHelpers.
+
+  Lemma bind_match {A B C D : Type} :
+    forall (x : option (A * B * C)) (f : C -> D),
+    match
+      match x with
+      | Some (a, v, g) => Some (a, v, f g)
+      | None => None
+      end
+    with
+    | Some (l, _, _) => Some l
+    | None => None
+    end
+    = match x with
+    | Some (a, v, g) => Some a
+    | None => None
+    end.
+  Proof.
+    intros x f.
+    (* Destruct x into None or Some p, then break the triple p into (a, (v, g)) *)
+    destruct x as [ [[a v] g] | ].
+    - (* Case: x = Some (a, v, g) *)
+      simpl. reflexivity.
+    - (* Case: x = None *)
+      simpl. reflexivity.
+  Qed.
+
+End MatchHelpers.
+
+(* Section InterpActionRewritesHelper.
+
+  Lemma rew_interp_action_code:
+    forall {reg_t: Type} {REnv: Env reg_t} {R: reg_t -> type} r sigma ctx log_r log_a e rest,
+      interp_action r sigma ctx log_r log_a (rew [fun _ => _] e in rest) = interp_action r sigma ctx log_r log_a rest.
+
+End InterpActionRewritesHelper. *)
