coq/Properties/Synthesis.v
@@ -1,0 +1,1457 @@
+Require Import Koika.Frontend.
+Require Import Koika.Std.
+Require Import Koika.Utils.Common.
+Require Import Koika.Utils.Environments.
+Require Export Koika.Primitives.
+
+Require Koika.Properties.SemanticProperties.
+
+Require Import Trustformer.Syntax.
+Require Import Trustformer.Semantics.
+Require Import Trustformer.Utils.
+Require Import Trustformer.Scheduler.Contract.
+Require Import Trustformer.TypedSynthesis.
+Require Trustformer.Properties.Common.
+From Koika.Utils Require Import Tactics.
+Require Import Koika.IRR.Tactics.
+
+Require Import Streams.
+Require Import Coq.Lists.List.
+Require Import Coq.Logic.Eqdep_dec.
+Require Import Coq.Init.Tactics.
+Require Import Coq.Setoids.Setoid.
+Require Import Coq.micromega.Lia.
+Require Import Coq.Program.Program.
+Require Import Coq.Program.Equality.
+Require Import Coq.Program.Tactics.
+
+Require Import Coq.Logic.ProofIrrelevance.
+
+Require Import Hammer.Plugin.Hammer.
+Set Hammer ATPLimit 5.
+Set Hammer GSMode 63.
+
+Section SynthesisCorrectness.
+
+  Context (tf_ctx: TFSynthContext).
+
+  (* ====== Abbreviations ====== *)
+  Local Notation sched_ctx := (tf_sched_ctx tf_ctx).
+  
+  Local Notation spec_states := (tfs_states (tf_sched_ctx tf_ctx)).
+  Local Notation spec_states_fin := (tfs_states_fin (tf_sched_ctx tf_ctx)).
+  Local Notation spec_states_size := (tfs_states_size (tf_sched_ctx tf_ctx)).
+  Local Notation spec_states_t := (tf_states_type spec_states_size).
+  Local Notation spec_states_init := (tfs_states_init (tf_sched_ctx tf_ctx)).
+  Local Notation spec_all_states := (@finite_elements spec_states spec_states_fin).
+  Local Notation spec_state_index := (@finite_index spec_states spec_states_fin).
+  Local Notation spec_state_num := (Datatypes.length spec_all_states).
+
+  Local Notation spec_inputs := (tfs_inputs (tf_sched_ctx tf_ctx)).
+  Local Notation spec_inputs_fin := (tfs_inputs_fin (tf_sched_ctx tf_ctx)).
+  Local Notation spec_inputs_size := (tfs_inputs_size (tf_sched_ctx tf_ctx)).
+  Local Notation spec_inputs_t := (tf_inputs_type spec_inputs_size).
+  Local Notation spec_all_inputs := (@finite_elements spec_inputs spec_inputs_fin).
+  Local Notation spec_input_index := (@finite_index spec_inputs spec_inputs_fin).
+  Local Notation spec_input_num := (Datatypes.length spec_all_inputs).
+
+  Local Notation spec_outputs := (tfs_outputs (tf_sched_ctx tf_ctx)).
+  Local Notation spec_outputs_fin := (tfs_outputs_fin (tf_sched_ctx tf_ctx)).
+  Local Notation spec_outputs_size := (tfs_outputs_size (tf_sched_ctx tf_ctx)).
+  Local Notation spec_outputs_t := (tf_outputs_type spec_outputs_size).
+  Local Notation spec_all_outputs := (@finite_elements spec_outputs spec_outputs_fin).
+  Local Notation spec_output_index := (@finite_index spec_outputs spec_outputs_fin).
+  Local Notation spec_output_num := (Datatypes.length spec_all_outputs).
+
+  Local Notation spec_action := (tfs_action (tf_sched_ctx tf_ctx)).
+  Local Notation spec_action_fin := (tfs_action_fin (tf_sched_ctx tf_ctx)).
+  Local Notation spec_all_actions := (@finite_elements spec_action spec_action_fin).
+  Local Notation spec_action_index := (@finite_index spec_action spec_action_fin).
+  Local Notation spec_action_num := (Datatypes.length spec_all_actions).
+
+  Local Notation spec_action_reg_size := (tf_action_reg_size tf_ctx).
+  Local Notation spec_action_encoding := (tf_action_encoding tf_ctx).
+  Local Notation spec_action_encoding_inj := (tf_action_encoding_inj tf_ctx).
+
+  Local Notation spec_schedule := (tfs_schedule (tf_sched_ctx tf_ctx)).
+  Local Notation spec_done_state := (tfs_done_signal (tf_sched_ctx tf_ctx)).
+  Local Notation spec_reset_states := (tfs_reset_states (tf_sched_ctx tf_ctx)).
+
+  Local Definition spec_schedule_ops_nodup := (tfs_schedule_no_duplicates (tf_sched_ctx tf_ctx)).
+
+  Local Notation reg_t := (@_reg_t spec_states spec_inputs spec_outputs).
+  Local Notation reg_t_finite := (@_reg_t_finite tf_ctx).
+  Local Notation ext_fn_t := (@_ext_fn_t spec_inputs spec_outputs).
+
+  Local Notation st_env := (ContextEnv.(env_t) (tf_states_type spec_states_size)).
+  Local Notation out_env := (ContextEnv.(env_t) (tf_outputs_type spec_outputs_size)).
+  Local Notation sys_state_t := (st_env * out_env)%type.
+  Local Notation input_t := (forall x : spec_inputs, type_denote (tf_inputs_type spec_inputs_size x)).
+
+  Local Notation R := (R tf_ctx).
+  Local Notation r := (r tf_ctx).
+  Local Notation Sigma := (Sigma tf_ctx).
+  Local Notation rules := (rules tf_ctx).
+  Local Notation system_schedule := (system_schedule tf_ctx).
+  Local Notation REnv := (@ContextEnv reg_t (_reg_t_finite tf_ctx)).
+
+  Hint Extern 0 (FiniteType spec_states) => exact (tfs_states_fin (tf_sched_ctx tf_ctx)) : typeclass_instances.
+  Hint Extern 0 (FiniteType spec_inputs) => exact (tfs_inputs_fin (tf_sched_ctx tf_ctx)) : typeclass_instances.
+  Hint Extern 0 (FiniteType spec_outputs) => exact (tfs_outputs_fin (tf_sched_ctx tf_ctx)) : typeclass_instances.
+  Hint Extern 0 (FiniteType spec_action) => exact (tfs_action_fin (tf_sched_ctx tf_ctx)) : typeclass_instances.
+
+  Hint Extern 0 (FiniteType reg_t) => exact (_reg_t_finite tf_ctx) : typeclass_instances.
+
+  Ltac match_eq :=
+  match goal with
+  | [ |- (match ?L with _ => _ end) = (match ?R with _ => _ end) ] =>
+    let LM := fresh "LM" in
+    let RM := fresh "RM" in
+    let HeqL := fresh "HeqLM" in
+    let HeqR := fresh "HeqRM" in
+    remember L as LM eqn:HeqL;
+    remember R as RM eqn:HeqR;
+    let H := fresh "H" in
+    assert (H : LM = RM); [ 
+      (* First subgoal: prove the scrutinees are equal *)
+      subst LM RM 
+    | (* Second subgoal: use the equality to close the original goal *)
+      rewrite H; reflexivity 
+    ]
+  end.
+
+  Ltac extract_match_term :=
+  match goal with
+  | |- context [match ?X with _ => _ end] =>
+      match X with
+      | context [match _ with _ => _ end] => 
+          fail 1
+      | _ => 
+          let MT := fresh "MT" in
+          let HeqMT := fresh "HeqMT" in
+          remember X as MT eqn:HeqMT
+      end
+  end.
+
+  Ltac in_match_term tac :=
+  match goal with
+  | |- context [match ?X with _ => _ end] =>
+      match X with
+      | context [match _ with _ => _ end] => 
+          fail 1
+      | _ => 
+          let MT := fresh "MT" in
+          let HeqMT := fresh "HeqMT" in
+          remember X as MT eqn:HeqMT;
+          tac HeqMT;
+          subst MT
+      end
+  end.
+
+  (* ====== Input Helper Lemmas ====== *)
+
+  Lemma nodup_spec_all_states : NoDup spec_all_states.
+  Proof. apply NoDup_map_inv with (f:=(finite_index (FiniteType:=spec_states_fin))). apply finite_injective. Qed.
+
+  Lemma nodup_spec_all_inputs : NoDup spec_all_inputs.
+  Proof. apply NoDup_map_inv with (f:=(finite_index (FiniteType:=spec_inputs_fin))). apply finite_injective. Qed.
+
+  Lemma nodup_spec_all_outputs : NoDup spec_all_outputs.
+  Proof. apply NoDup_map_inv with (f:=(finite_index (FiniteType:=spec_outputs_fin))). apply finite_injective. Qed.
+
+  Lemma nodup_spec_all_actions : NoDup spec_all_actions.
+  Proof. apply NoDup_map_inv with (f:=(finite_index (FiniteType:=spec_action_fin))). apply finite_injective. Qed.
+
+  Lemma in_spec_all_states : forall x, In x spec_all_states.
+  Proof. 
+    intros x. generalize (finite_surjective x (FiniteType:=spec_states_fin)). 
+    intros H1. apply nth_error_In with (finite_index x (FiniteType:=spec_states_fin)). exact H1. 
+  Qed.
+
+  Lemma in_spec_all_inputs : forall x, In x spec_all_inputs.
+  Proof. 
+    intros x. generalize (finite_surjective x (FiniteType:=spec_inputs_fin)). 
+    intros H1. apply nth_error_In with (finite_index x (FiniteType:=spec_inputs_fin)). exact H1. 
+  Qed.
+
+  Lemma in_spec_all_outputs : forall x, In x spec_all_outputs.
+  Proof. 
+    intros x. generalize (finite_surjective x (FiniteType:=spec_outputs_fin)). 
+    intros H1. apply nth_error_In with (finite_index x (FiniteType:=spec_outputs_fin)). exact H1. 
+  Qed.
+
+  Lemma in_spec_all_actions : forall x, In x spec_all_actions.
+  Proof. 
+    intros x. generalize (finite_surjective x (FiniteType:=spec_action_fin)). 
+    intros H1. apply nth_error_In with (finite_index x (FiniteType:=spec_action_fin)). exact H1. 
+  Qed.
+
+  Lemma not_in_reg_ready_all_states:
+    ~ In (tf_ready (states_var:=spec_states) (inputs_var:=spec_inputs) (outputs_var:=spec_outputs)) (map tf_reg spec_all_states).
+  Proof.
+    intro. rewrite in_map_iff in H. destruct H as [x [Heq Hin]]. congruence.
+  Qed.
+
+  Lemma not_in_reg_ready_all_outputs:
+    ~ In (tf_ready (states_var:=spec_states) (inputs_var:=spec_inputs) (outputs_var:=spec_outputs)) (map tf_out spec_all_outputs).
+  Proof.
+    intro. rewrite in_map_iff in H. destruct H as [x [Heq Hin]]. congruence.
+  Qed.  
+
+  Lemma not_in_reg_cmd_all_states:
+    ~ In (tf_cmd (states_var:=spec_states) (inputs_var:=spec_inputs) (outputs_var:=spec_outputs)) (map tf_reg spec_all_states).
+  Proof.
+    intro. rewrite in_map_iff in H. destruct H as [x [Heq Hin]]. congruence.
+  Qed.
+
+  Lemma not_in_reg_cmd_all_outputs:
+    ~ In (tf_cmd (states_var:=spec_states) (inputs_var:=spec_inputs) (outputs_var:=spec_outputs)) (map tf_out spec_all_outputs).
+  Proof.
+    intro. rewrite in_map_iff in H. destruct H as [x [Heq Hin]]. congruence.
+  Qed.
+
+  Lemma not_in_reg_reg_all_inputs:
+    forall x, ~ In (tf_reg (states_var:=spec_states) (inputs_var:=spec_inputs) (outputs_var:=spec_outputs) x) (map tf_in spec_all_inputs).
+  Proof.
+    intro. intro. rewrite in_map_iff in H. destruct H as [x0 [Heq Hin]]. subst. congruence.
+  Qed.
+
+  Lemma not_in_reg_out_all_inputs:
+    forall x, ~ In (tf_out (states_var:=spec_states) (inputs_var:=spec_inputs) (outputs_var:=spec_outputs) x) (map tf_in spec_all_inputs).
+  Proof.
+    intro. intro. rewrite in_map_iff in H. destruct H as [x0 [Heq Hin]]. subst. congruence.
+  Qed.
+
+  Lemma not_in_reg_ready_all_inputs:
+    ~ In (tf_ready (states_var:=spec_states) (inputs_var:=spec_inputs) (outputs_var:=spec_outputs)) (map tf_in spec_all_inputs).
+  Proof.
+    intro. rewrite in_map_iff in H. destruct H as [x [Heq Hin]]. congruence.
+  Qed.
+
+  Section Encoding.
+
+    Lemma spec_action_encoding_inj' :
+      forall (a1 a2 : spec_action),
+      a1 <> a2 -> spec_action_encoding a1 <> spec_action_encoding a2.
+    Proof.
+      intros a1 a2 H_neq. intros H_eq.
+      apply spec_action_encoding_inj in H_eq.
+      contradiction.
+    Qed.    
+
+    Lemma reg_name_inj :
+      forall r1 r2,
+        (_reg_name tf_ctx r1) = (_reg_name tf_ctx r2) -> r1 = r2.
+    Proof.
+      intros. unfold _reg_name in H.
+      timeout 10 simpl in H. 
+      injection H. intros.
+      apply string_id_of_nat_inj in H0.
+      apply finite_index_injective in H0.
+      exact H0.
+    Qed.
+
+    Lemma reg_name_inj' :
+      forall r1 r2,
+        (_reg_name tf_ctx r1) <> (_reg_name tf_ctx r2) -> r1 <> r2.
+    Proof.
+      intros. unfold _reg_name in H.
+      timeout 10 simpl in H.
+      unfold not in *. intros. subst r2.
+      apply H. reflexivity.
+    Qed.
+
+    Lemma out_name_inj :
+      forall o1 o2,
+        (_out_name tf_ctx o1) = (_out_name tf_ctx o2) -> o1 = o2.
+    Proof.
+      intros. unfold _out_name in H.
+      timeout 10 simpl in H.
+      injection H. intros.
+      apply string_id_of_nat_inj in H0.
+      apply finite_index_injective in H0.
+      exact H0.
+    Qed.
+
+    Lemma out_name_inj' :
+      forall o1 o2,
+        (_out_name tf_ctx o1) <> (_out_name tf_ctx o2) -> o1 <> o2.
+    Proof.
+      intros. unfold _out_name in H.
+      timeout 10 simpl in H. 
+      unfold not in *. intros. subst o2.
+      apply H. reflexivity.
+    Qed.
+
+    Lemma reg_ready_or_not (r: ContextEnv.(env_t) R) :
+      { r.[tf_ready] = Ob~1 } + { r.[tf_ready] = Ob~0 }.
+    Proof.
+      destruct (eq_dec r.[tf_ready] (Ob~1)) as [Hready | Hnotready'].
+      - left. assumption.
+      - right.
+        destruct r.[tf_ready] eqn:Hready_val; try discriminate.
+        vm_compute Bits.of_nat in *. destruct vtl; try discriminate.
+        destruct vhd; try reflexivity. contradiction.
+    Qed.
+
+  End Encoding. 
+
+  Opaque _register_var_name.
+
+  (* ====== State and Environment Relations ====== *)
+
+  Definition state_matches (sys: sys_state_t) (r: ContextEnv.(env_t) R) : Prop :=
+    (* State variables map cleanly *)
+    (forall (x: spec_states), r.[tf_reg x] = (fst sys).[x]) /\
+    (* Output variables map cleanly *)
+    (forall (x: spec_outputs), r.[tf_out x] = (snd sys).[x]).
+
+  Definition state_equal (r1 r2: ContextEnv.(env_t) R): Prop :=
+    (forall (x: spec_states), r1.[tf_reg x] = r2.[tf_reg x]) /\
+    (forall (x: spec_outputs), r1.[tf_out x] = r2.[tf_out x]).
+
+  Definition env_matches (act: spec_action) (input: input_t) (r: ContextEnv.(env_t) R) : Prop :=
+    (* action variable maps cleanly *)
+    (r.[tf_cmd] = spec_action_encoding act) /\
+    (* input variables map cleanly *)
+    (forall (x: spec_inputs), r.[tf_in x] = input x).
+
+  Definition env_equal (r1 r2: ContextEnv.(env_t) R): Prop :=
+    (r1.[tf_cmd] = r2.[tf_cmd]) /\
+    (forall (x: spec_inputs), r1.[tf_in x] = r2.[tf_in x]).
+
+  Definition state_env_matches (sys: sys_state_t) (act: spec_action) (input: input_t) (r: ContextEnv.(env_t) R) : Prop :=
+    state_matches sys r /\
+    env_matches act input r.
+
+  Definition input_matches (act: spec_action) (input: input_t) (sigma: forall f, Sig_denote (Sigma f)) : Prop :=
+    let cmd_res := sigma ext_in_cmd Ob~1 in      
+    (fst cmd_res) = Ob~1 /\ (* TODO: implicit params should be given explicitly once known *)
+    (@fst (vect bool (tf_action_reg_size tf_ctx)) unit
+      (@snd (vect_cons_t bool (vect_nil_t bool)) (prod (vect bool (tf_action_reg_size tf_ctx)) unit) cmd_res) = spec_action_encoding act) /\
+    (forall (x: spec_inputs), sigma (ext_input x) (Ob~1) = input x).
+
+  (* Lemma state_env_matches_comp :
+    forall sys act input r1 r2,
+      state_equal r1 r2 ->
+      env_equal r1 r2 ->
+      state_env_matches sys act input r1 = state_env_matches sys act input r2.
+  Proof.
+    intros. 
+    unfold state_equal in H. destruct H as [Hstate_eq Hout_eq].
+    unfold env_equal in H0. destruct H0 as [Hcmd_eq Hin_eq].
+    unfold state_env_matches, state_matches, env_matches. f_equal; [f_equal | f_equal].
+    (* - apply prop_ext.  *) (* Not provable without function extensionality *)
+
+  Admitted.  *)
+
+  (* ====== Initial State Correctness ====== *)
+
+  Definition abstract_init_state (sys: sys_state_t) : Prop :=
+    (forall x, (fst sys).[x] = spec_states_init x) /\
+    (forall x, (snd sys).[x] = Bits.zero).
+
+  Theorem initial_state_matches :
+    forall (sys: sys_state_t),
+      abstract_init_state sys ->
+      state_matches sys ((ContextEnv).(create) r).
+  Proof.
+    intros sys Hinit.
+    unfold state_matches, abstract_init_state in *.
+    destruct Hinit as [Hstate Houtput].
+    split; intros x.
+    - rewrite getenv_create. simpl. symmetry. apply Hstate.
+    - rewrite getenv_create. simpl. symmetry. apply Houtput.
+  Qed.
+
+  (* ====== Translation Validation ====== *)
+
+  Arguments log_empty : simpl never.
+  Arguments log_cons : simpl never.
+
+  Section MayReadWrite.
+
+    Local Notation may_read := (may_read (R:=R) (REnv:=REnv) (reg_t:=reg_t)).
+    Local Notation may_write := (may_write (R:=R) (REnv:=REnv) (reg_t:=reg_t)).
+
+    Lemma may_read0_implies_may_read1 :
+      forall log_r idx,
+        may_read log_r P0 idx = true -> may_read log_r P1 idx = true.
+    Proof.
+      intros log_r idx H. unfold may_read in *. apply andb_prop in H. destruct H as [H_is_write0 H_is_write1]. exact H_is_write1.
+    (* Time Qed. *)
+    Admitted. (* SPEEDUP *)
+    (* 15 seconds *)
+
+    Lemma may_write0_implies_may_write1 :
+      forall log_r log_a idx,
+        may_write log_r log_a P0 idx = true -> may_write log_r log_a P1 idx = true.
+    Proof.
+      intros log_r log_a idx H. unfold may_write in *. apply andb_prop in H. destruct H as [H_cons H_is_write1].
+      exact H_is_write1.
+    (* Time Qed. *)
+    Admitted. (* SPEEDUP *)
+    (* ??? seconds *)
+
+    Definition may_read_all log_r port regs :=
+      forallb (may_read log_r port) regs.
+
+    Definition may_write_all log_r log_a port regs :=
+      forallb (may_write log_r log_a port) regs.
+
+    Lemma may_read_all0_implies_may_read_all1 :
+      forall log_r regs,
+        may_read_all log_r P0 regs = true -> may_read_all log_r P1 regs = true.
+    Proof.
+      intros log_r regs H. unfold may_read_all in *. rewrite forallb_forall in H. apply forallb_forall. intros x Hin.
+      apply H in Hin. apply may_read0_implies_may_read1. exact Hin.
+    Qed.
+
+    Lemma may_write_log_cons_neq :
+      forall log_r log_a port
+             idx1 idx2 entry,
+        idx2 <> idx1 ->
+        may_write log_r (log_cons idx1 entry log_a) port idx2
+        = may_write log_r log_a port idx2.
+    Proof.
+      intros log_r log_a port idx1 idx2 entry Hneq. destruct entry, kind.
+      + unfold may_write. rewrite !SemanticProperties.log_existsb_app.
+        rewrite !(SemanticProperties.log_existsb_log_cons_neq log_a idx2 idx1); try assumption; reflexivity.
+      + unfold may_write. rewrite !SemanticProperties.log_existsb_app.
+        rewrite !(SemanticProperties.log_existsb_log_cons_neq log_a idx2 idx1); try assumption; reflexivity.
+    Qed.
+
+    Lemma may_write_log_cons_eq :
+      forall log_r log_a prt
+             idx entry,
+        may_write log_r (log_cons idx entry log_a) prt idx
+        = may_write log_r log_a prt idx && 
+          match prt with
+          | P0 =>
+            negb (is_read1 (kind entry) (port entry)) 
+            && negb (is_write0 (kind entry) (port entry))
+            && negb (is_write1 (kind entry) (port entry))
+          | P1 => negb (is_write1 (kind entry) (port entry))
+          end.
+    Proof.
+      intros log_r log_a prt idx entry. destruct entry, kind.
+      - unfold may_write. rewrite !SemanticProperties.log_existsb_app.
+        rewrite !(SemanticProperties.log_existsb_log_cons_eq log_a idx).
+        destruct prt; simpl.
+        + destruct port; simpl; [ rewrite andb_true_r | rewrite andb_false_r ]; reflexivity.
+        + rewrite andb_true_r; reflexivity.
+      - unfold may_write. rewrite !SemanticProperties.log_existsb_app.
+        rewrite !(SemanticProperties.log_existsb_log_cons_eq log_a idx).
+        destruct prt; simpl.
+        + destruct port; simpl; rewrite !andb_false_r; reflexivity.
+        + destruct port; simpl; [ rewrite andb_true_r | rewrite andb_false_r ]; reflexivity.
+    Qed.
+
+    Lemma may_write_all_log_cons_neq :
+      forall log_r log_a port regs
+             idx entry,
+        ~ In idx regs ->
+        may_write_all log_r (log_cons idx entry log_a) port regs
+        = may_write_all log_r log_a port regs.
+    Proof.
+      intros log_r log_a port regs idx entry Hnotin.
+      unfold may_write_all. apply forallb_pointwise. intros.
+      assert (x <> idx) as Hx_neq.
+      { intros Heq. subst x. contradiction. }
+      rewrite may_write_log_cons_neq; try assumption. reflexivity.
+    Qed.
+
+    Lemma may_write_all_log_cons :
+      forall log_r log_a prt regs
+             idx entry,
+        In idx regs ->
+        may_write_all log_r (log_cons idx entry log_a) prt regs
+        = may_write_all log_r log_a prt regs && 
+          match prt with
+          | P0 =>
+            negb (is_read1 (kind entry) (port entry)) 
+            && negb (is_write0 (kind entry) (port entry))
+            && negb (is_write1 (kind entry) (port entry))
+          | P1 => negb (is_write1 (kind entry) (port entry))
+          end.
+    Proof.
+      intros log_r log_a prt regs idx entry Hin.
+
+      induction regs as [| r regs H0 ]; simpl in *; try contradiction.
+      destruct Hin as [Heq | Hin]; subst.
+      - destruct (Common.in_dec idx regs).
+        + rewrite (H0 i). rewrite may_write_log_cons_eq.
+          destruct prt; simpl.
+          * remember ((negb _) && (negb _) && (negb _)) as cond.
+            destruct cond; [ rewrite !andb_true_r | rewrite !andb_false_r ]; reflexivity.
+          * destruct negb; [ rewrite !andb_true_r | rewrite !andb_false_r ]; reflexivity.
+        + rewrite may_write_all_log_cons_neq by assumption. rewrite may_write_log_cons_eq.
+          rewrite <- !andb_assoc. rewrite (andb_comm (may_write_all _ _ _ _)). reflexivity.
+      - rewrite (H0 Hin); clear H0 Hin.
+        destruct (eq_dec r idx) as [Heq | Hneq]; subst.
+        + rewrite may_write_log_cons_eq. 
+          destruct prt; simpl.
+          * remember ((negb _) && (negb _) && (negb _)) as cond.
+            destruct cond; [ rewrite !andb_true_r | rewrite !andb_false_r ]; reflexivity.
+          * destruct negb; [ rewrite !andb_true_r | rewrite !andb_false_r ]; reflexivity.
+        + rewrite may_write_log_cons_neq by assumption. rewrite andb_assoc. reflexivity.
+    Qed.
+
+    Lemma may_write_all_cons :
+      forall log1 log2 P0 r regs,
+      may_write_all log1 log2 P0 (r :: regs) = true ->
+      may_write log1 log2 P0 r = true /\ may_write_all log1 log2 P0 regs = true.
+    Proof.
+      intros log1 log2 P0 r regs H.
+      unfold may_write_all in H. simpl in H.
+      apply andb_prop in H. destruct H as [H_r H_regs].
+      split; assumption.
+    Qed.
+
+    Lemma may_read_all_cons :
+      forall log1 P0 r regs,
+      may_read_all log1 P0 (r :: regs) = true ->
+      may_read log1 P0 r = true /\ may_read_all log1 P0 regs = true.
+    Proof.
+      intros log1 P0 r regs H.
+      unfold may_read_all in H. simpl in H.
+      apply andb_prop in H. destruct H as [H_r H_regs].
+      split; assumption.
+    Qed.
+
+  End MayReadWrite.
+
+  Arguments may_read : simpl never.
+  Arguments may_write : simpl never.
+  Arguments may_write_all : simpl never.
+  Arguments may_read_all : simpl never.
+
+  Local Notation Write0 x := ({| kind := LogWrite; port := P0; val := x |}).
+  Local Notation Write1 x := ({| kind := LogWrite; port := P1; val := x |}).
+  Local Notation Read0 := ({| kind := LogRead; port := P0; val := tt |}).
+  Local Notation Read1 := ({| kind := LogRead; port := P1; val := tt |}).
+
+  Section Interpreting.
+
+    (* Goal: Write stepper lemmas for simplifying the interp_rule below *)
+
+    Local Notation interp_action := (interp_action (reg_t:=reg_t) (pos_t:=pos_t) (var_t:=var_t) (fn_name_t:=fn_name_t) (R:=R) (Sigma:=Sigma) (REnv:=REnv)).
+
+    Lemma interp_action_seq :
+      forall r sigma sig (ctx: tcontext sig) log_r log_a a1 a2,
+        interp_action (tau:=unit_t) r sigma ctx log_r log_a (Seq a1 a2) = 
+          let/opt3 log_a, _, Gamma := interp_action r sigma ctx log_r log_a a1 
+          in interp_action r sigma Gamma log_r log_a a2.
+    Proof. reflexivity. Qed.
+
+    Lemma interp_action_if :
+      forall r sigma sig (ctx: tcontext sig) log_r log_a cond tbranch fbranch,
+        interp_action (tau:=unit_t) r sigma ctx log_r log_a (If cond tbranch fbranch) = 
+          let/opt3 log_a, cond0, Gamma := interp_action r sigma ctx log_r log_a cond
+          in (if Bits.single cond0 
+              then interp_action r sigma Gamma log_r log_a tbranch 
+              else interp_action r sigma Gamma log_r log_a fbranch).
+    Proof. reflexivity. Qed.
+
+    Lemma interp_action_read0 :
+      forall r sigma sig (ctx: tcontext sig) log_r log_a idx,
+        may_read log_r P0 idx = true ->
+        interp_action (tau:=R idx) r sigma ctx log_r log_a (Read P0 idx) = 
+        Some (log_cons idx {| kind := LogRead; port := P0; val := tt |} log_a, r.[idx], ctx).
+    Proof. intros; simpl. rewrite H; try auto. Qed.
+
+    Lemma interp_action_buffer_inputs_cons :
+      forall r_env sigma log1 log2 i inputs rest,
+        may_write log1 log2 P0 (tf_in i) = true ->
+        interp_action (tau:=unit_t) r_env sigma CtxEmpty log1 log2 (rule_buffer_inputs tf_ctx (i :: inputs) rest) =
+        interp_action r_env sigma CtxEmpty log1
+            (log_cons (tf_in i) (Write0 (sigma (ext_input i) Ob~1)) log2)
+            (rule_buffer_inputs tf_ctx inputs rest)
+        .
+    Proof.
+      intros. simpl. rewrite H. reflexivity.
+    Time Qed.
+
+  End Interpreting.
+
+  Lemma interp_action_buffer_inputs :
+    forall (r: ContextEnv.(env_t) R) (input: input_t)
+           (sigma: forall f, Sig_denote (Sigma f))
+           log1 log2 rest,
+      (forall x : spec_inputs, sigma (ext_input x) Ob~1 = input x) ->
+      may_write_all log1 log2 P0 (map tf_in spec_all_inputs) = true ->
+
+      interp_action (tau:=unit_t) r sigma CtxEmpty log1 log2 (rule_buffer_inputs tf_ctx spec_all_inputs rest) = 
+      let log_n := fold_left (fun log x => log_cons (tf_in x) (Write0 (sigma (ext_input x) Ob~1)) log) spec_all_inputs log2 in
+      interp_action r sigma CtxEmpty log1 log_n rest.
+  Proof.
+    intros r input sigma log1 log2 rest Hinput Hwr0_in.
+
+    pose proof (nodup_spec_all_inputs) as H_nodup_inputs.
+    generalize dependent log2. generalize rest.
+
+    induction spec_all_inputs as [| i inputs H0 ]; intros.
+    - reflexivity.
+    - cbn [map] in Hwr0_in. apply may_write_all_cons in Hwr0_in; destruct Hwr0_in as [Hwr0_i Hwr0_inputs].
+      rewrite interp_action_buffer_inputs_cons; try assumption.
+      cbn [fold_left]. apply (H0); clear H0.
+      + abstract ( inversion H_nodup_inputs; subst; assumption ).
+      + rewrite may_write_all_log_cons_neq; try assumption.
+        apply Common.not_in_map; try assumption.
+        * abstract ( inversion H_nodup_inputs; subst; assumption ).
+        * abstract ( intros; inversion H; reflexivity ).
+  (* Timeout 600 Time Qed.  *)
+  Admitted. (* SPEEDUP *)
+  (* 12 seconds *)    
+
+  Lemma may_write_fold_cons_w0_inputs :
+    forall log log2 prt x (sigma: forall f, Sig_denote (Sigma f)),
+    ~ In x (map tf_in spec_all_inputs) ->
+    may_write log (fold_left (fun log x => log_cons (tf_in x) (Write0 (sigma (ext_input x) Ob~1)) log) spec_all_inputs log2) prt x
+    = may_write (R:=R) (REnv:=REnv) log log2 prt x.
+  Proof.
+    intros log log2 prt x sigma Hnotin.
+
+    assert (NoDup (map (tf_in (states_var:=spec_states) (inputs_var:=spec_inputs) (outputs_var:=spec_outputs)) (rev spec_all_inputs))) as Hnodup.
+    { 
+      rewrite map_rev. apply NoDup_rev. apply FinFun.Injective_map_NoDup. 
+      + unfold FinFun.Injective. intros. (* hammer *) timeout 10 sfirstorder.
+      + apply nodup_spec_all_inputs.
+    }
+
+    rewrite in_rev in *. rewrite <- map_rev in *.
+    rewrite <- fold_left_rev_right. 
+    
+    induction (rev spec_all_inputs) as [| i inputs H0 ]; simpl in *.
+    - reflexivity.
+    - apply Decidable.not_or in Hnotin. destruct Hnotin as [Hnotin_i Hnotin_inputs].
+      rewrite may_write_log_cons_neq; try (symmetry; assumption). apply H0; clear H0; try assumption.
+      inversion Hnodup. subst. exact H2.
+  Qed.
+
+  Lemma may_write_all_fold_cons_w0_inputs :
+    forall log log2 prt (sigma: forall f, Sig_denote (Sigma f)) l,
+    (forall x, In x l -> ~ In x (map tf_in spec_all_inputs)) ->
+    may_write_all log (fold_left (fun log x => log_cons (tf_in x) (Write0 (sigma (ext_input x) Ob~1)) log) spec_all_inputs log2) prt l
+    = may_write_all log log2 prt l.
+  Proof.
+    intros log log2 prt sigma l Hnot_in.
+
+    unfold may_write_all. apply forallb_pointwise. intros.
+    rewrite may_write_fold_cons_w0_inputs; try assumption.
+    - reflexivity.
+    - apply (Hnot_in x H).
+  Qed.
+
+  Definition log_after_cmd_guard_rdy (act: spec_action) (sigma: forall f, Sig_denote (Sigma f)) :=
+    log_cons (R:=R) (REnv:=REnv) tf_ready (Write0 Ob~0)
+      (log_cons tf_cmd (Write0 (spec_action_encoding act))
+        (fold_left
+          (fun log0 x => log_cons (tf_in x) (Write0 (sigma (ext_input x) Ob~1)) log0) 
+            spec_all_inputs (log_cons tf_ready Read0 (log_cons tf_ready Read0 (log_cons tf_ready Read0 log_empty))))).
+
+  Lemma interp_action_cmd_guard :
+    forall (sys: sys_state_t) (r: ContextEnv.(env_t) R) 
+           (act: spec_action) (input: input_t)
+           (sigma: forall f, Sig_denote (Sigma f))
+           log,
+      state_matches sys r ->
+      ( r.[tf_ready] = Ob~1 -> input_matches act input sigma ) ->
+      ( r.[tf_ready] = Ob~0 -> env_matches act input r ) ->
+      may_write_all log log_empty P0 (map tf_in spec_all_inputs) = true ->
+      may_read log P0 (tf_ready) = true ->
+      may_write log log_empty P0 (tf_ready) = true ->
+      may_read log P0 (tf_cmd) = true ->
+      may_write log log_empty P0 (tf_cmd) = true ->
+      interp_action r sigma CtxEmpty log log_empty (rule_cmd_guard tf_ctx act) = 
+      Some ( 
+        if Bits.single r.[tf_ready] then log_after_cmd_guard_rdy act sigma else log_cons tf_cmd Read0 (log_cons tf_ready Read0 log_empty),
+        Ob,
+        CtxEmpty
+      ).
+  Proof.
+    intros sys r act input sigma log Hstate Hinput_rdy Hinput_nrdy.
+    intros Hwr0_in Hrd0_rdy Hwr0_ready Hrd0_cmd Hwr0_cmd.
+
+    unfold rule_cmd_guard. rewrite interp_action_if. 
+    (* Set Printing Implicit. *) change (bits_t 1) with (R tf_ready) at 2. rewrite interp_action_read0; try assumption.
+    unfold opt_bind.
+    
+    destruct (reg_ready_or_not r) as [Hready | Hnotready].
+    - (* Ready case *)
+      in_match_term ltac:(fun H => rewrite Hready in H; cbn in H).
+
+      rewrite interp_action_seq. unfold Guard. rewrite interp_action_if.
+      unfold opt_bind. extract_match_term. cbn in HeqMT. rewrite Hrd0_rdy in HeqMT. cbn in HeqMT.
+      subst MT. 
+      
+      unfold input_matches in Hinput_rdy. destruct Hinput_rdy as [Hval [Hcmd Hinput]]; try assumption.
+      rewrite Hready. extract_match_term. setoid_rewrite Hval in HeqMT. cbn in HeqMT. subst MT.
+
+      in_match_term ltac:(fun H => cbn in H).
+      rewrite interp_action_seq. rewrite interp_action_if. unfold opt_bind.
+
+      extract_match_term. cbn in HeqMT. rewrite Hrd0_rdy in HeqMT. rewrite Hready in HeqMT. cbn in HeqMT. 
+      unfold BitFuns._eq in HeqMT. rewrite Hcmd in HeqMT. rewrite beq_dec_refl in HeqMT.
+      subst MT.
+
+      in_match_term ltac:(fun H => cbn in H).
+      in_match_term ltac:(fun H => cbn in H).
+      rewrite (interp_action_buffer_inputs r input sigma).
+      + rewrite interp_action_seq. 
+        unfold opt_bind. in_match_term ltac:(fun H => cbn in H).
+      
+        rewrite may_write_fold_cons_w0_inputs.
+        2: { intro. rewrite in_map_iff in H. destruct H as [x [Heq Hin]]. congruence. }
+
+        set (MW := may_write _ _ P0 tf_cmd). assert (MW = true) as HMW.
+        { subst MW. rewrite !may_write_log_cons_neq; try assumption. all: (* hammer *) timeout 10 sauto. } rewrite HMW. clear HMW MW.
+        cbn.
+
+        set (MW := may_write _ _ P0 tf_ready). assert (MW = true) as HMW.
+        { 
+          subst MW. rewrite !may_write_log_cons_neq; [|(* hammer *) timeout 10 sauto]. rewrite may_write_fold_cons_w0_inputs. 
+          2: { intro. rewrite in_map_iff in H. destruct H as [x [Heq Hin]]. congruence. }
+          rewrite !may_write_log_cons_eq. rewrite Hwr0_ready. ring. 
+        } rewrite HMW. clear HMW MW.
+        unfold log_after_cmd_guard_rdy. reflexivity.
+      + exact Hinput.
+      + rewrite !may_write_all_log_cons_neq. exact Hwr0_in.
+        all: abstract (intro; rewrite in_map_iff in H; destruct H as [x [Heq Hin]]; subst; congruence).
+    - (* Not ready case *)
+      in_match_term ltac:(fun H => rewrite Hnotready in H; cbn in H).
+      unfold Guard. rewrite interp_action_if. unfold opt_bind. 
+      in_match_term ltac:(fun H => cbn in H; rewrite Hrd0_cmd in H; cbn in H).
+
+      unfold env_matches in Hinput_rdy. destruct Hinput_nrdy as [Hcmd Hin]; try assumption.
+      extract_match_term. rewrite Hcmd in HeqMT. cbn in HeqMT. rewrite beq_dec_refl in HeqMT. subst MT.
+      reflexivity.
+  (* Timeout 600 Time Qed.  *)
+  Admitted. (* SPEEDUP *)
+  (* 188 seconds *)
+
+  Program Fixpoint CtxReadVars (r: ContextEnv.(env_t) R) (regs: list reg_t) (sig: tsig var_t) (acc: tcontext sig) : 
+    tcontext (rev (map (fun r => (_register_var_name tf_ctx r, R r)) regs) ++ sig) :=
+    match regs with
+    | [] => acc
+    | reg :: rs => 
+        let k_tau := (_register_var_name tf_ctx reg, R reg) in
+        CtxReadVars r rs (k_tau :: sig) (CtxCons k_tau (r.[reg]) acc)
+    end.
+  Next Obligation.
+    rewrite <- List.app_assoc.
+    reflexivity.
+  Qed.
+
+  Arguments _Log : simpl never.
+
+
+  Lemma interp_action_read_vars_states:
+    forall r sigma tau sig
+      (rest : action R Sigma (rev (map (fun r => (_register_var_name tf_ctx r, R r)) (map tf_reg spec_all_states)) ++ sig) tau)
+      log_r log_a (ctx: tcontext (var_t:=var_t) sig),
+      may_read_all log_r P0 (map tf_reg spec_all_states) = true ->
+        match 
+          interp_action r sigma 
+            ctx 
+            log_r log_a 
+            (rule_read_vars tf_ctx (_register_var_name tf_ctx) (map tf_reg spec_all_states) rest)
+        return option (Log R REnv) with
+        | Some (l, _, _) => Some (l)
+        | None => None
+        end =
+        match 
+          interp_action r sigma 
+            (CtxReadVars r (map tf_reg spec_all_states) sig ctx) log_r 
+            (fold_left (fun log s => log_cons (tf_reg s) (LE LogRead P0 tt) log) spec_all_states log_a) rest
+        return option (Log R REnv) with
+        | Some (l, _, _) => Some (l)
+        | None => None
+        end.
+  Proof.
+    intros r sigma tau sig rest log_r log_a ctx Hrd0_st.
+
+
+    (* pose proof (nodup_spec_all_states) as H_nodup_all_states. *)
+    generalize dependent log_a. generalize dependent rest. generalize dependent tau. generalize dependent ctx. generalize dependent sig.
+
+    induction spec_all_states as [| s states H0 ]; intros.
+    - reflexivity.
+    - cbn in Hrd0_st. apply may_read_all_cons in Hrd0_st; destruct Hrd0_st as [Hrd0_s Hrd0_states].
+      specialize (H0 Hrd0_states). 
+      cbn. rewrite Hrd0_s. cbn. unfold opt_bind.
+      rewrite Common.bind_match.
+
+      rewrite H0; clear H0. clear.
+      admit. (* Dependent Type Hell *)
+      
+      (* set (e := TypedSynthesis.rule_read_vars_obligation_1 _ _ _ _ _).
+      set (e0 := CtxReadVars_obligation_1 _ _ _).
+      clearbody e e0. cbv zeta in e, e0.
+
+      dependent destruction e. dependent destruction e0.  *)
+   
+  Admitted.
+
+  Lemma interp_action_read_vars_outputs:
+    forall r sigma tau sig
+      (rest : action R Sigma (rev (map (fun r => (_register_var_name tf_ctx r, R r)) (map tf_out spec_all_outputs)) ++ sig) tau)
+      log_r log_a (ctx: tcontext (var_t:=var_t) sig),
+      may_read_all log_r P0 (map tf_out spec_all_outputs) = true ->
+        match interp_action r sigma ctx log_r log_a 
+          (rule_read_vars tf_ctx (_register_var_name tf_ctx) (map tf_out spec_all_outputs) rest)
+        return option (Log R REnv) with
+        | Some (l, _, _) => Some (l)
+        | None => None
+        end =
+        match 
+          interp_action r sigma (CtxReadVars r (map tf_out spec_all_outputs) sig ctx) log_r 
+            (fold_left (fun log s => log_cons (tf_out s) (LE LogRead P0 tt) log) spec_all_outputs log_a) rest
+        return option (Log R REnv) with
+        | Some (l, _, _) => Some (l)
+        | None => None
+        end.
+  Proof.
+    intros r sigma tau sig rest log_r log_a ctx Hrd0_out.
+
+    generalize dependent log_a. generalize dependent rest. generalize dependent tau. generalize dependent ctx. generalize dependent sig.
+
+    induction spec_all_outputs as [| s outputs H0 ]; intros.
+    - reflexivity.
+    - cbn in Hrd0_out. apply may_read_all_cons in Hrd0_out; destruct Hrd0_out as [Hrd0_s Hrd0_outputs].
+      specialize (H0 Hrd0_outputs). 
+      cbn. rewrite Hrd0_s. cbn. unfold opt_bind.
+      rewrite Common.bind_match.
+
+      rewrite H0; clear H0. clear.
+      admit. (* Dependent Type Hell *)
+  Admitted.
+
+  Fixpoint eval_expr_aux {szB}
+      (expr: tf_expr) log
+      (sys_state: sys_state_t)
+      (input: input_t)
+      : (bits_t szB * list reg_t) :=
+        match expr with
+        | tf_const value =>
+            (Bits.of_nat szB value, log)
+        | tf_svar v =>
+            (convert (fst sys_state).[v], tf_reg v :: log)
+        | tf_ivar v =>
+            (convert (input v), tf_in v :: log)
+        | tf_ovar v =>
+            (convert (snd sys_state).[v], tf_out v :: log)
+        | tf_op1 op src =>
+            let (val_src, log_src) := (eval_expr_aux src log sys_state input) in
+            (
+              match op with
+              | tf_not => Bits.neg val_src
+              end,
+              log_src
+            )
+        | tf_op2 op src1 src2 =>
+            let (val_src1, log_src1) := (eval_expr_aux src1 log sys_state input) in
+            let (val_src2, log_src2) := (eval_expr_aux src2 log_src1 sys_state input) in
+            match op with
+            | tf_and => (Bits.and val_src1 val_src2, log_src2)
+            | tf_or => (Bits.or val_src1 val_src2, log_src2)
+            | tf_xor => (Bits.xor val_src1 val_src2, log_src2)
+            | tf_add => (Bits.plus val_src1 val_src2, log_src2)
+            | tf_sub => (Bits.minus val_src1 val_src2, log_src2)
+            | tf_mul => (convert (Bits.mul val_src1 val_src2), log_src2)
+            | tf_cmp szC cmp_op =>
+                let (val_cmp_src1, log_cmp_src1) := (eval_expr_aux (szB:=szC) src1 log_src2 sys_state input) in
+                let (val_cmp_src2, log_cmp_src2) := (eval_expr_aux (szB:=szC) src2 log_cmp_src1 sys_state input) in
+                (
+                  match cmp_op with
+                  | tf_eq =>
+                      if beq_dec val_cmp_src1 val_cmp_src2 then Bits.of_nat szB 1 else Bits.of_nat szB 0
+                  | tf_neq =>
+                      if beq_dec val_cmp_src1 val_cmp_src2 then Bits.of_nat szB 0 else Bits.of_nat szB 1
+                  | tf_lt =>
+                      if Bits.unsigned_lt val_cmp_src1 val_cmp_src2 then Bits.of_nat szB 1 else Bits.of_nat szB 0
+                  | tf_le =>
+                      if Bits.unsigned_le val_cmp_src1 val_cmp_src2 then Bits.of_nat szB 1 else Bits.of_nat szB 0
+                  | tf_gt =>
+                      if Bits.unsigned_gt val_cmp_src1 val_cmp_src2 then Bits.of_nat szB 1 else Bits.of_nat szB 0
+                  | tf_ge =>
+                      if Bits.unsigned_ge val_cmp_src1 val_cmp_src2 then Bits.of_nat szB 1 else Bits.of_nat szB 0
+                  end,
+                  log_cmp_src2
+                )
+            end
+        | tf_expr_if cond then_expr else_expr =>
+            let (val_cond, log_cond) := (eval_expr_aux (szB:=1) cond log sys_state input) in
+            if beq_dec val_cond Bits.zero then (* Note: we check for false i.e. all bits are zero, thus the bodies here are switched *)
+              eval_expr_aux else_expr log_cond sys_state input 
+            else
+              eval_expr_aux then_expr log_cond sys_state input
+        end.
+
+  Definition expr_log (expr: tf_expr) (szB: nat) (sys_state: sys_state_t) (input: input_t) log :=
+    fold_left (fun acc reg => log_cons (R:=R) (REnv:=REnv) reg {| kind := LogRead; port := match reg with
+                                                   | tf_in v => P1
+                                                   | _ => P0
+                                                   end; val := tt |} acc ) (snd (eval_expr_aux (szB:=szB) expr [] sys_state input)) log.
+
+  (* 
+  TODO: here
+  
+  Lemma interp_synth_convert :
+    forall r sigma log_r log_a szA ctx sig szB (expr : action R Sigma sig (bits_t szA)),
+      interp_action (R:=R) (REnv:=REnv) r sigma ctx log_r log_a (synth_convert (in_var_size := szA) tf_ctx szB expr) = 
+      match interp_action (R:=R) (REnv:=REnv) r sigma ctx log_r log_a expr 
+      return option (Log R REnv * bits_t szB * sig) with
+      | Some (l, v, g) => Some (l, convert (szB:=szB) v, g)
+      | None => None
+      end.
+  Proof.
+    intros r sigma log_r log_a szB szA expr.
+
+    unfold synth_convert. 
+    generalize dependent expr.
+    (* Dependent Type Hell *)
+    (* destruct (lt_eq_lt_dec szA szB) as [[Hlt | Hlt] | Hgt]; intros. *)
+    admit.
+  Admitted. *)
+
+  Lemma interp_action_expr :
+    forall (sys: sys_state_t) (r: ContextEnv.(env_t) R) 
+           (act: spec_action) (input: input_t)
+           (sigma: forall f, Sig_denote (Sigma f))
+           log_r log_a expr dst,
+      state_matches sys r ->
+      env_matches act input r ->
+      interp_action r sigma
+        (CtxReadVars r (map tf_out spec_all_outputs) (rev (map (fun r0 : reg_t => (_register_var_name tf_ctx r0, R r0)) (map tf_reg spec_all_states)) ++ [])
+        (CtxReadVars r (map tf_reg spec_all_states) [] CtxEmpty)) log_r log_a (expr_to_action tf_ctx expr (spec_states_size dst))
+      = Some (
+          expr_log expr (spec_states_size dst) sys input log_a, 
+          tf_eval_expr (szB:=spec_states_size dst) spec_states_size spec_inputs_size spec_outputs_size expr sys input, 
+          CtxReadVars r (map tf_out spec_all_outputs) (rev (map (fun r0 : reg_t => (_register_var_name tf_ctx r0, R r0)) (map tf_reg spec_all_states)) ++ [])
+          (CtxReadVars r (map tf_reg spec_all_states) [] CtxEmpty)
+        ).
+  Proof.
+    intros sys r act input sigma log_r log_a expr dst.
+    intros Hstate Hinput_rdy.
+
+    induction expr.
+    + (* Const *)
+      reflexivity.
+    + (* Var *)
+      cbn. rewrite interp_synth_convert. reflexivity.
+      
+      admit. 
+
+  Definition affected_regs (ops: list (@tf_op spec_states spec_inputs spec_outputs)) : list reg_t :=
+    fold_right (fun op acc => match op with
+                             | tf_assign dst _ => tf_reg dst :: acc
+                             | tf_output dst _ => tf_out dst :: acc
+                             | _ => acc
+                             end) [] ops.
+
+  Lemma interp_action_aux :
+    forall (sys: sys_state_t) (r: ContextEnv.(env_t) R) 
+           (act: spec_action) (input: input_t)
+           (sigma: forall f, Sig_denote (Sigma f))
+           log_r log_a ops rest,
+      state_matches sys r ->
+      env_matches act input r ->
+      may_read_all log_r P1 (map tf_in spec_all_inputs) = true ->
+      NoDup (affected_regs ops) ->
+      may_write_all log_r log_a P0 (affected_regs ops) = true ->
+      match interp_action (tau:=unit_t) r sigma (CtxReadVars r (map tf_out spec_all_outputs) (rev (map (fun r0 : reg_t => (_register_var_name tf_ctx r0, R r0)) (map tf_reg spec_all_states)) ++ [])
+                                    (CtxReadVars r (map tf_reg spec_all_states) [] CtxEmpty))
+              log_r log_a (rule_aux tf_ctx ops rest)
+      return option (Log R REnv) with
+      | Some (l, _, _) => Some (l)
+      | None => None
+      end =
+      None.
+  Proof.
+    intros r sigma log_r log_a ops rest.
+    intros Hrd1_in HNoDup_aff Hwr0_aff.
+
+    generalize dependent log_a. generalize dependent rest.
+    induction ops as [| op ops H0 ]; intros.
+    - admit.
+    - destruct op.
+      + cbn. apply H0; [ exact HNoDup_aff | exact Hwr0_aff ].
+      + cbn. cbn in Hwr0_aff. apply may_write_all_cons in Hwr0_aff. destruct Hwr0_aff as [Hwr0_dst Hwr0_rest].
+        admit.
+        (* rewrite Hwr0_dst. apply H0; [| exact Hwr0_rest]. *)
+  Admitted.
+
+  Definition construct_log (sys: sys_state_t) (act: spec_action) (input: input_t) ready (log_a: Log R ContextEnv): Log R ContextEnv :=
+    let updates := if 
+                    beq_dec (find_st_val sched_ctx spec_done_state (tfs_get_updates sched_ctx (fst (spec_schedule act)) sys input) sys) Bits.zero
+                  then 
+                    tfs_get_updates sched_ctx (fst (spec_schedule act)) sys input
+                  else 
+                    tfs_reset_updates sched_ctx spec_reset_states 
+                    ++ tfs_get_updates sched_ctx (snd (spec_schedule act)) sys input 
+                    ++ tfs_get_updates sched_ctx (fst (spec_schedule act)) sys input in
+    match eq_dec ready Ob~1 with
+    | left Hready => log_a (* TODO: update while working on the proof below *)
+    | right Hnotready => log_a (* TODO: update while working on the proof below *)
+    end.
+
+  Lemma interp_action_cmd :
+    forall (sys: sys_state_t) (r: ContextEnv.(env_t) R) 
+           (act: spec_action) (input: input_t)
+           (sigma: forall f, Sig_denote (Sigma f))
+           log_r log_a,
+      state_matches sys r ->
+      env_matches act input r ->
+      may_read_all log_r P0 (map tf_reg spec_all_states) = true ->
+      may_write_all log_r log_a P0 (map tf_reg spec_all_states) = true ->
+      may_read_all log_r P1 (map tf_in spec_all_inputs) = true ->
+      may_read_all log_r P0 (map tf_out spec_all_outputs) = true ->
+      may_write_all log_r log_a P0 (map tf_out spec_all_outputs) = true ->
+      may_write log_r log_a P1 (tf_ready) = true ->
+      match interp_action r sigma CtxEmpty log_r log_a (_rule_cmd tf_ctx act) with
+      | Some (l, v, _) => Some (l)
+      | None => None
+      end =
+      Some ( construct_log sys act input r.[tf_ready] log_a ).
+  Proof.
+    intros sys r act input sigma log_r log_a Hstate Hinput_rdy Hinput_nrdy.
+    intros Hrd0_st Hwr0_st Hrd1_in Hrd0_out Hwr0_out Hwr1_ready.
+    
+    unfold _rule_cmd. rewrite interp_action_read_vars_states; try assumption.
+    rewrite interp_action_read_vars_outputs; try assumption.
+    admit.
+  Admitted.
+
+  Lemma interp_rule_correct :
+    forall (sys: sys_state_t) (r: ContextEnv.(env_t) R) 
+           (act: spec_action) (input: input_t)
+           (sigma: forall f, Sig_denote (Sigma f))
+           log,
+      state_matches sys r ->
+      ( r.[tf_ready] = Ob~1 -> input_matches act input sigma ) ->
+      ( r.[tf_ready] = Ob~0 -> env_matches act input r ) ->
+      may_read_all log P0 (map tf_reg spec_all_states) = true ->
+      may_write_all log log_empty P0 (map tf_reg spec_all_states) = true ->
+      may_read_all log P0 (map tf_in spec_all_inputs) = true ->
+      may_write_all log log_empty P0 (map tf_in spec_all_inputs) = true ->
+      may_read_all log P0 (map tf_out spec_all_outputs) = true ->
+      may_write_all log log_empty P0 (map tf_out spec_all_outputs) = true ->
+      may_read log P0 (tf_ready) = true ->
+      may_write log log_empty P0 (tf_ready) = true ->
+      may_read log P0 (tf_cmd) = true ->
+      may_write log log_empty P0 (tf_cmd) = true ->
+      let guard_log := if Bits.single r.[tf_ready] then log_after_cmd_guard_rdy act sigma else log_cons tf_cmd Read0 (log_cons tf_ready Read0 log_empty) in
+      interp_rule r sigma log (rules (rule_cmd act)) = Some (construct_log sys act input r.[tf_ready] guard_log).
+  Proof.
+    intros sys r act input sigma log Hstate Hinput_rdy Hinput_nrdy.
+    intros Hrd0_st Hwr0_st Hrd0_in Hwr0_in Hrd0_out Hwr0_out Hrd0_rdy Hwr0_ready Hrd0_cmd Hwr0_cmd.
+    unfold interp_rule, rules.
+
+    rewrite interp_action_seq. unfold opt_bind.
+    rewrite (interp_action_cmd_guard sys r act input sigma log); try assumption.
+
+    setoid_rewrite (interp_action_cmd sys r act input sigma log 
+              (if Bits.single r.[tf_ready] 
+                then log_after_cmd_guard_rdy act sigma 
+                else log_cons tf_cmd Read0 (log_cons tf_ready Read0 log_empty))).
+    - reflexivity.
+    - assumption.
+    - assumption.
+    - assumption.
+    - assumption.
+    - destruct (reg_ready_or_not r) as [Hready | Hnotready].
+      + rewrite Hready. cbn. unfold log_after_cmd_guard_rdy. 
+        rewrite !may_write_all_log_cons_neq. rewrite may_write_all_fold_cons_w0_inputs. rewrite !may_write_all_log_cons_neq. assumption.
+        all: (try exact not_in_reg_ready_all_states); (try exact not_in_reg_cmd_all_states).
+        intros. rewrite in_map_iff in H. destruct H as [x0 [Heq Hin]]. subst. exact (not_in_reg_reg_all_inputs x0).
+      + rewrite Hnotready. cbn. rewrite !may_write_all_log_cons_neq. assumption.
+        all: (try exact not_in_reg_ready_all_states); (try exact not_in_reg_cmd_all_states).
+    - apply may_read_all0_implies_may_read_all1. assumption.  
+    - assumption.
+    - destruct (reg_ready_or_not r) as [Hready | Hnotready].
+      + rewrite Hready. cbn. unfold log_after_cmd_guard_rdy. 
+        rewrite !may_write_all_log_cons_neq. rewrite may_write_all_fold_cons_w0_inputs. rewrite !may_write_all_log_cons_neq. assumption.
+        all: (try exact not_in_reg_ready_all_outputs); (try exact not_in_reg_cmd_all_outputs).
+        intros. rewrite in_map_iff in H. destruct H as [x0 [Heq Hin]]. subst. exact (not_in_reg_out_all_inputs x0).
+      + rewrite Hnotready. cbn. rewrite !may_write_all_log_cons_neq. assumption.
+        all: (try exact not_in_reg_ready_all_outputs); (try exact not_in_reg_cmd_all_outputs).
+    - destruct (reg_ready_or_not r) as [Hready | Hnotready].
+      + rewrite Hready. cbn. unfold log_after_cmd_guard_rdy.
+        rewrite may_write_log_cons_eq. rewrite may_write_log_cons_neq. 
+        rewrite may_write_fold_cons_w0_inputs. rewrite !may_write_log_cons_eq. simpl. rewrite !andb_true_r.
+        * apply may_write0_implies_may_write1. assumption. 
+        * exact not_in_reg_ready_all_inputs. 
+        * intro. congruence.
+      + rewrite Hnotready. cbn. rewrite may_write_log_cons_neq. rewrite may_write_log_cons_eq. simpl. rewrite !andb_true_r.
+        * apply may_write0_implies_may_write1. assumption.
+        * intro. congruence.
+  (* Time Qed. *)
+  Admitted. (* SPEEDUP *)
+  (* ??? seconds *)
+
+  (* 
+    Once we can substitue the expensive HW interpretation with a contructed log, we should be able to work on the lemmas below
+    until then we do not wish to proceed past this point
+  *)
+Abort.
+
+  Lemma latest_write_cmd_rdy :
+    forall (sys: sys_state_t) (r: ContextEnv.(env_t) R) 
+           (act: spec_action) (input: input_t)
+           (sigma: forall f, Sig_denote (Sigma f))
+           log,
+      state_matches sys r ->
+      ( r.[tf_ready] = Ob~1 -> input_matches act input sigma ) ->
+      ( r.[tf_ready] = Ob~0 -> env_matches act input r ) ->
+      good_log log ->
+      r.[tf_ready] = Ob~1 ->
+      latest_write match interp_rule r sigma log (rules (rule_cmd act)) with
+        | Some l => log_app l log
+        | None => log
+        end tf_cmd = Some (spec_action_encoding act).
+  Proof.
+  Admitted.
+
+  Lemma latest_write_cmd_nrdy :
+    forall (sys: sys_state_t) (r: ContextEnv.(env_t) R) 
+           (act: spec_action) (input: input_t)
+           (sigma: forall f, Sig_denote (Sigma f))
+           log,
+      state_matches sys r ->
+      ( r.[tf_ready] = Ob~1 -> input_matches act input sigma ) ->
+      ( r.[tf_ready] = Ob~0 -> env_matches act input r ) ->
+      good_log log ->
+      r.[tf_ready] = Ob~0 ->
+      latest_write match interp_rule r sigma log (rules (rule_cmd act)) with
+        | Some l => log_app l log
+        | None => log
+        end tf_cmd = None.
+  Proof.
+  Admitted.
+
+  Lemma latest_write_input_rdy :
+    forall (sys: sys_state_t) (r: ContextEnv.(env_t) R) 
+           (act: spec_action) (input: input_t)
+           (sigma: forall f, Sig_denote (Sigma f))
+           log x,
+      state_matches sys r ->
+      ( r.[tf_ready] = Ob~1 -> input_matches act input sigma ) ->
+      ( r.[tf_ready] = Ob~0 -> env_matches act input r ) ->
+      good_log log ->
+      r.[tf_ready] = Ob~1 ->
+      latest_write match interp_rule r sigma log (rules (rule_cmd act)) with
+        | Some l => log_app l log
+        | None => log
+        end (tf_in x) = Some (input x).
+  Proof.
+  Admitted.
+
+  Lemma latest_write_input_nrdy :
+    forall (sys: sys_state_t) (r: ContextEnv.(env_t) R) 
+           (act: spec_action) (input: input_t)
+           (sigma: forall f, Sig_denote (Sigma f))
+           log x,
+      state_matches sys r ->
+      ( r.[tf_ready] = Ob~1 -> input_matches act input sigma ) ->
+      ( r.[tf_ready] = Ob~0 -> env_matches act input r ) ->
+      good_log log ->
+      r.[tf_ready] = Ob~0 ->
+      latest_write match interp_rule r sigma log (rules (rule_cmd act)) with
+        | Some l => log_app l log
+        | None => log
+        end (tf_in x) = None.
+  Proof.
+  Admitted.
+
+  Lemma latest_write_reg :
+    forall (sys: sys_state_t) (r: ContextEnv.(env_t) R) 
+           (act: spec_action) (input: input_t)
+           (sigma: forall f, Sig_denote (Sigma f))
+           log x,
+      state_matches sys r ->
+      ( r.[tf_ready] = Ob~1 -> input_matches act input sigma ) ->
+      ( r.[tf_ready] = Ob~0 -> env_matches act input r ) ->
+      good_log log ->
+      latest_write match interp_rule r sigma log (rules (rule_cmd act)) with
+        | Some l => log_app l log
+        | None => log
+        end (tf_reg x) =
+        find_st_update sched_ctx x
+          (if 
+            beq_dec (find_st_val sched_ctx spec_done_state (tfs_get_updates sched_ctx (fst (spec_schedule act)) sys input) sys) Bits.zero
+          then 
+            tfs_get_updates sched_ctx (fst (spec_schedule act)) sys input
+          else 
+            tfs_reset_updates sched_ctx spec_reset_states 
+            ++ tfs_get_updates sched_ctx (snd (spec_schedule act)) sys input 
+            ++ tfs_get_updates sched_ctx (fst (spec_schedule act)) sys input).
+  Proof.
+  Admitted.
+
+  Lemma latest_write_out :
+    forall (sys: sys_state_t) (r: ContextEnv.(env_t) R) 
+           (act: spec_action) (input: input_t)
+           (sigma: forall f, Sig_denote (Sigma f))
+           log x,
+      state_matches sys r ->
+      ( r.[tf_ready] = Ob~1 -> input_matches act input sigma ) ->
+      ( r.[tf_ready] = Ob~0 -> env_matches act input r ) ->
+      good_log log ->
+      latest_write match interp_rule r sigma log (rules (rule_cmd act)) with
+        | Some l => log_app l log
+        | None => log
+        end (tf_out x) =
+        find_out_update sched_ctx x
+          (if 
+            beq_dec (find_st_val sched_ctx spec_done_state (tfs_get_updates sched_ctx (fst (spec_schedule act)) sys input) sys) Bits.zero
+          then 
+            tfs_get_updates sched_ctx (fst (spec_schedule act)) sys input
+          else 
+            tfs_reset_updates sched_ctx spec_reset_states 
+            ++ tfs_get_updates sched_ctx (snd (spec_schedule act)) sys input 
+            ++ tfs_get_updates sched_ctx (fst (spec_schedule act)) sys input).
+  Proof.
+  Admitted.
+
+  Lemma synthesis_correct_aux3 :
+    forall (sys: sys_state_t) (r: ContextEnv.(env_t) R) 
+           (act: spec_action) (input: input_t)
+           (sigma: forall f, Sig_denote (Sigma f))
+           log,
+      state_matches sys r ->
+      ( r.[tf_ready] = Ob~1 -> input_matches act input sigma ) ->
+      ( r.[tf_ready] = Ob~0 -> env_matches act input r ) ->
+      good_log log ->
+      state_env_matches (tfs_next_cycle sched_ctx act sys input) act input (commit_update r match interp_rule r sigma log (rules (rule_cmd act)) with
+        | Some l => log_app l log
+        | None => log
+        end).
+  Proof.
+    intros sys r act input sigma log Hstate Hin_rdy Hin_nrdy Hlog.
+    unfold state_env_matches; split.
+    - unfold state_matches; split; intros.
+      + unfold commit_update, tfs_next_cycle. cbn [fst snd].
+        rewrite !getenv_create. unfold find_st_val at 1.
+        assert (r.[tf_reg x] = (fst sys).[x]) as Hreg. { apply Hstate. } rewrite Hreg. clear Hreg.
+        match_eq. apply latest_write_reg; try assumption.
+      + unfold commit_update, tfs_next_cycle. cbn [fst snd].
+        rewrite !getenv_create. unfold find_out_val at 1.
+        assert (r.[tf_out x] = (snd sys).[x]) as Hreg. { apply Hstate. } rewrite Hreg. clear Hreg.
+        match_eq. apply latest_write_out; try assumption.
+    - unfold env_matches; split; intros.
+      + unfold commit_update. rewrite getenv_create.
+        destruct (reg_ready_or_not r) as [Hready | Hnotready].
+        * rewrite (latest_write_cmd_rdy sys r act input sigma log); try assumption; reflexivity.
+        * rewrite (latest_write_cmd_nrdy sys r act input sigma log); try assumption. apply (Hin_nrdy Hnotready). auto.
+      + unfold commit_update. rewrite getenv_create.
+        destruct (reg_ready_or_not r) as [Hready | Hnotready].
+        * rewrite (latest_write_input_rdy sys r act input sigma log x); try assumption; reflexivity.
+        * rewrite (latest_write_input_nrdy sys r act input sigma log x); try assumption. apply (Hin_nrdy Hnotready). 
+  Qed.
+
+  Lemma interp_rule_cmd_wrong :
+    forall (sys: sys_state_t) (r: ContextEnv.(env_t) R) 
+           (act: spec_action) (input: input_t)
+           (sigma: forall f, Sig_denote (Sigma f))
+           log a,
+      state_matches sys r ->
+      ( r.[tf_ready] = Ob~1 -> input_matches act input sigma ) ->
+      ( r.[tf_ready] = Ob~0 -> env_matches act input r ) ->
+      act <> a ->
+      interp_rule r sigma log (rules (rule_cmd a)) = None.
+  Proof.
+    intros sys r act input sigma log a Hstate Hin_rdy Hin_nrdy Hact_neq_a.
+    unfold interp_rule, rules, rule_cmd_guard. simpl_eq. (* Takes a while, but otherwise qed stalls *)
+    destruct may_read; try reflexivity. timeout 10 cbn. 
+    destruct (reg_ready_or_not r) as [Hready | Hnotready].
+    - specialize (Hin_rdy Hready) as H_in. rewrite Hready. timeout 10 cbn.
+      destruct Bits.single; try reflexivity. timeout 10 cbn. destruct beq_dec eqn:Hbeq; try reflexivity.
+      apply beq_dec_iff in Hbeq. contradict Hbeq.
+      unfold input_matches in H_in. destruct H_in as [H_v [H_act_enc H_input]].
+      rewrite H_act_enc. apply spec_action_encoding_inj'. assumption.
+    - specialize (Hin_nrdy Hnotready) as H_in. rewrite Hnotready. timeout 10 cbn.
+      destruct may_read; try reflexivity. timeout 10 cbn. destruct beq_dec eqn:Hbeq; try reflexivity.
+      apply beq_dec_iff in Hbeq. contradict Hbeq.
+      unfold env_matches in H_in. destruct H_in as [H_cmd _]. rewrite H_cmd; try auto.
+      apply spec_action_encoding_inj'. assumption.
+  Qed.  
+
+  Lemma latest_write_schedule_outputs :
+    forall (r: ContextEnv.(env_t) R) (sigma: forall f, Sig_denote (Sigma f)) log x,
+      match x with | tf_out_ack _ => False | _ => True end ->
+      latest_write (interp_scheduler' r sigma rules log (system_schedule_outputs tf_ctx)) x = latest_write log x.
+  Proof.
+    intros r sigma log x Hx. unfold system_schedule_outputs.
+
+    assert (forall t, tf_out_ack t <> x). { intros t. (* hammer *) sfirstorder. } clear Hx.
+    
+    generalize dependent log.
+    induction (spec_all_outputs) as [|o outputs IH]; intros log.
+    - cbn [fold_right interp_scheduler']. destruct x; reflexivity.
+    - cbn [fold_right interp_scheduler' rules]. unfold interp_rule. cbn [interp_action].
+      unfold opt_bind. destruct may_read; [|apply IH]. destruct may_write; [rewrite IH|apply IH]. 
+      clear IH. rewrite SemanticProperties.latest_write_app. 
+      rewrite SemanticProperties.latest_write_cons_neq; [|symmetry; exact (H o)].
+      rewrite Common.latest_write_log_cons_read; [|auto].
+      rewrite SemanticProperties.latest_write_empty. reflexivity.
+  Qed.
+
+  Lemma synthesis_correct_aux2 :
+    forall (sys: sys_state_t) (r: ContextEnv.(env_t) R) 
+           (act: spec_action) (input: input_t)
+           (sigma: forall f, Sig_denote (Sigma f))
+           log (actions: list spec_action),
+      state_matches sys r ->
+      ( r.[tf_ready] = Ob~1 -> input_matches act input sigma ) ->
+      ( r.[tf_ready] = Ob~0 -> env_matches act input r ) ->
+      good_log log ->
+      ~ In act actions ->
+      state_env_matches (tfs_next_cycle sched_ctx act sys input) act input
+        (commit_update r
+          match interp_rule r sigma log (rules (rule_cmd act)) with
+          | Some l => interp_scheduler' r sigma rules (log_app l log) (fold_right (fun (t : spec_action) (acc : scheduler) => rule_cmd t |> acc) (system_schedule_outputs tf_ctx) actions)
+          | None => interp_scheduler' r sigma rules log (fold_right (fun (t : spec_action) (acc : scheduler) => rule_cmd t |> acc) (system_schedule_outputs tf_ctx) actions)
+          end)
+      =
+      state_env_matches (tfs_next_cycle sched_ctx act sys input) act input (commit_update r
+          match interp_rule r sigma log (rules (rule_cmd act)) with
+          | Some l => (log_app l log)
+          | None => log
+          end).
+  Proof.
+    intros sys r act input sigma log actions Hstate Hin_rdy Hin_nrdy Hlog H_notin_actions.
+
+    induction actions as [|a actions IH].
+    - cbn [fold_right]. 
+      apply state_env_matches_comp;
+        (* All: *) unfold state_equal, env_equal; split;
+          (* All: *) intros x; unfold commit_update; rewrite !getenv_create; match_eq; destruct interp_rule; apply latest_write_schedule_outputs; reflexivity.
+    - apply not_in_cons in H_notin_actions. destruct H_notin_actions as [Hneq Hnotin].
+
+      cbn [fold_right interp_scheduler'].
+      destruct (interp_rule r sigma log (rules (rule_cmd act))) as [l | ] eqn:H_interp_cmd.
+      + rewrite (interp_rule_cmd_wrong sys r act input sigma (log_app l log) a Hstate Hin_rdy Hin_nrdy); try assumption.
+        apply IH; try assumption.
+      + rewrite (interp_rule_cmd_wrong sys r act input sigma log a Hstate Hin_rdy Hin_nrdy); try assumption.
+        apply IH; try assumption.
+  Qed.
+
+
+  Lemma synthesis_correct_aux :
+    forall (sys: sys_state_t) (r: ContextEnv.(env_t) R) 
+           (act: spec_action) (input: input_t)
+           (sigma: forall f, Sig_denote (Sigma f))
+           log,
+      state_matches sys r ->
+      ( r.[tf_ready] = Ob~1 -> input_matches act input sigma ) ->
+      ( r.[tf_ready] = Ob~0 -> env_matches act input r ) ->
+      good_log log ->
+      state_env_matches (tfs_next_cycle sched_ctx act sys input) act input (commit_update r (interp_scheduler' r sigma rules log (system_schedule_actions tf_ctx))).
+  Proof.
+    intros sys r act input sigma log Hstate Hin_rdy Hin_nrdy Hlog.
+    unfold system_schedule_actions.
+
+    pose proof (nodup_spec_all_actions) as H_nodup_actions.
+    pose proof (in_spec_all_actions act) as H_in_actions.
+
+    generalize dependent log.
+    induction (spec_all_actions) as [|a actions IH] ; [inversion H_in_actions | ]. intros log Hlog.
+    
+    apply NoDup_cons_iff in H_nodup_actions. destruct H_nodup_actions as [H_a_notin H_nodup_actions].
+    destruct H_in_actions as [H_act_eq | H_in_actions]; subst.
+
+    - (* current action is the requested action *)
+      cbn [fold_right interp_scheduler'].
+
+      rewrite synthesis_correct_aux2; try assumption.
+      apply (synthesis_correct_aux3 sys r act input sigma log Hstate Hin_rdy Hin_nrdy Hlog).
+
+    - (* current action is not the requested action *)
+      assert (H_act_neq_a: act <> a). { intro H. subst. contradiction. }
+      cbn [fold_right interp_scheduler'].
+
+      rewrite (interp_rule_cmd_wrong sys r act input sigma log a Hstate Hin_rdy Hin_nrdy H_act_neq_a).
+      apply IH; try assumption.
+  Qed.
+
+  Lemma interp_rule_busy_ready : 
+    forall (r: ContextEnv.(env_t) R) sigma,
+      r.[tf_ready] = Ob~1 ->
+      interp_rule r sigma log_empty (rules rule_busy) = None.
+  Proof.
+    intros r sigma Hready. unfold rules, interp_rule. unfold interp_action. 
+    rewrite Hready. destruct may_read; sauto.
+  Qed.
+
+  Lemma interp_rule_busy_not_ready : 
+    forall (r: ContextEnv.(env_t) R) sigma,
+      r.[tf_ready] = Ob~0 ->
+      interp_rule r sigma log_empty (rules rule_busy) = Some (
+        log_cons tf_cmd_ack {| kind := LogWrite; port := P0; val := fst (sigma ext_in_cmd (getenv ContextEnv r tf_ready)) |}
+          (log_cons tf_ready {| kind := LogRead; port := P0; val := tt |} 
+            (log_cons tf_ready {| kind := LogRead; port := P0; val := tt |} 
+              log_empty)
+          )
+        ).
+  Proof.
+    intros r sigma Hready. unfold rules, interp_rule, interp_action. 
+    rewrite Hready. simpl_eq.
+
+    (* prove we may read *)
+    set (mr := may_read _ _ _). assert (mr = true). 
+    { subst mr. unfold may_read. rewrite !SemanticProperties.log_existsb_empty. sauto. }
+    rewrite H. clear H mr.
+    
+    unfold opt_bind.
+    set (cond := Bits.single _). cbn in cond. subst cond. cbv iota.
+    
+    (* prove we may write *)
+    set (mw := may_write _ _ _ _). assert (mw = true). 
+    { 
+      subst mw. unfold may_write. rewrite !SemanticProperties.log_existsb_app. rewrite !Common.log_existsb_cons. rewrite !SemanticProperties.log_existsb_empty.
+      (* hammer *) timeout 10 hauto.
+    }
+    rewrite H, Hready. reflexivity.
+  Qed.
+ 
+  Theorem synthesis_correct :
+    forall (sys: sys_state_t) (r: ContextEnv.(env_t) R) 
+           (act: spec_action) (input: input_t)
+           (sigma: forall f, Sig_denote (Sigma f)),
+      state_matches sys r ->
+      ( r.[tf_ready] = Ob~1 -> input_matches act input sigma ) ->
+      ( r.[tf_ready] = Ob~0 -> env_matches act input r ) ->
+      state_env_matches (tfs_next_cycle sched_ctx act sys input) act input (interp_cycle sigma rules system_schedule r).
+  Proof.
+    intros sys r act input sigma Hstate Hin_rdy Hin_nrdy.
+    
+    unfold interp_cycle, interp_scheduler, system_schedule in *.
+    cbn [interp_scheduler'].
+
+    (* case destinction on whether hardware is ready or not *)
+    destruct (reg_ready_or_not r) as [Hready | Hnotready].
+    - specialize (Hin_rdy Hready) as H_in.
+      
+      (* simplify the busy rule *)
+      specialize (interp_rule_busy_ready r sigma Hready) as H_busy_ready. 
+      rewrite H_busy_ready. clear H_busy_ready.
+
+      apply synthesis_correct_aux; try assumption.
+      (* Show that the log is good *)
+      exact log_empty_good_log.
+
+    - specialize (Hin_nrdy Hnotready) as H_in.
+
+      (* simplify the busy rule *)
+      specialize (interp_rule_busy_not_ready r sigma Hnotready) as H_busy_not_ready.
+      rewrite H_busy_not_ready. clear H_busy_not_ready.
+
+      apply synthesis_correct_aux; try assumption.
+      (* Show that the log is good *)
+      apply good_log_app; try exact log_empty_good_log.
+      apply good_log_cons. apply good_log_cons. apply good_log_cons.
+      all: try exact log_empty_good_log; try timeout 10 sauto.
+  Qed.
+
+End SynthesisCorrectness.
